@prefix : <https://w3id.org/transmodel/facilities#> .
@prefix owl: <http://www.w3.org/2002/07/owl#> .
@prefix rdf: <http://www.w3.org/1999/02/22-rdf-syntax-ns#> .
@prefix xml: <http://www.w3.org/XML/1998/namespace> .
@prefix xsd: <http://www.w3.org/2001/XMLSchema#> .
@prefix rdfs: <http://www.w3.org/2000/01/rdf-schema#> .
@base <https://w3id.org/transmodel/facilities#> .

<https://w3id.org/transmodel/facilities#> rdf:type owl:Ontology ;
                                           owl:versionIRI <https://w3id.org/transmodel/facilities/0.2> ;
                                           <http://creativecommons.org/ns#license> <http://creativecommons.org/licenses/by/4.0/> ;
                                           <http://purl.org/dc/elements/1.1/creator> "Adolfo Antón Bravo (Ontology Engineering Group - Universidad Politécnica de Madrid)" ,
                                                                                     "Oscar Corcho (Ontology Engineering Group - Universidad Politécnica de Madrid)" ;
                                           <http://purl.org/dc/elements/1.1/date> "2019-10-06" ;
                                           <http://purl.org/dc/elements/1.1/description> "Module of the Transmodel Ontology focused on facilities. This ontology provides support to the NeTEx model. Visit https://github.com/oeg-upm/transmodel-ontology"@en ;
                                           <http://purl.org/dc/elements/1.1/identifier> "https://w3id.org/transmodel/facilities" ;
                                           <http://purl.org/dc/elements/1.1/rights> "Creative Commons Attribution 4.0 International (CC BY 4.0)" ;
                                           <http://purl.org/dc/elements/1.1/title> "Transmodel Ontology - Facilities"@en ;
                                           <http://purl.org/vocab/vann/preferredNamespaceUri> <https://w3id.org/transmodel/facilities#> ;
                                           rdfs:comment "Module of the Transmodel Ontology focused on facilities. This ontology provides support to the NeTEx model. Visit https://github.com/oeg-upm/transmodel-ontology"@en ;
                                           rdfs:label "Transmodel Ontology - Facilities"@en ;
                                           rdfs:seeAlso "https://github.com/oeg-upm/transmodel-ontology"@en ;
                                           owl:versionInfo "This is the initial version of the module on Facilities, after considering the UML models and XSD descriptions of Transmodel and NeTEx"@en .

#################################################################
#    Annotation properties
#################################################################

###  http://creativecommons.org/ns#license
<http://creativecommons.org/ns#license> rdf:type owl:AnnotationProperty .


###  http://purl.org/dc/elements/1.1/creator
<http://purl.org/dc/elements/1.1/creator> rdf:type owl:AnnotationProperty .


###  http://purl.org/dc/elements/1.1/date
<http://purl.org/dc/elements/1.1/date> rdf:type owl:AnnotationProperty .


###  http://purl.org/dc/elements/1.1/description
<http://purl.org/dc/elements/1.1/description> rdf:type owl:AnnotationProperty .


###  http://purl.org/dc/elements/1.1/identifier
<http://purl.org/dc/elements/1.1/identifier> rdf:type owl:AnnotationProperty .


###  http://purl.org/dc/elements/1.1/rights
<http://purl.org/dc/elements/1.1/rights> rdf:type owl:AnnotationProperty .


###  http://purl.org/dc/elements/1.1/title
<http://purl.org/dc/elements/1.1/title> rdf:type owl:AnnotationProperty .


###  http://purl.org/vocab/vann/preferredNamespaceUri
<http://purl.org/vocab/vann/preferredNamespaceUri> rdf:type owl:AnnotationProperty .


###  https://w3id.org/transmodel/facilities#author
:author rdf:type owl:AnnotationProperty .


###  https://w3id.org/transmodel/facilities#creator
:creator rdf:type owl:AnnotationProperty .


###  https://w3id.org/transmodel/facilities#description
:description rdf:type owl:AnnotationProperty ;
             rdfs:range rdfs:Literal ;
             rdfs:domain :MeetingPointService .


###  https://w3id.org/transmodel/facilities#mbox
:mbox rdf:type owl:AnnotationProperty .


###  https://w3id.org/transmodel/facilities#name
:name rdf:type owl:AnnotationProperty ;
      rdfs:range rdfs:Literal .


#################################################################
#    Datatypes
#################################################################

###  http://www.w3.org/2001/XMLSchema#duration
xsd:duration rdf:type rdfs:Datatype .


###  http://www.w3.org/2001/XMLSchema#string
xsd:string owl:equivalentClass xsd:duration .


#################################################################
#    Object Properties
#################################################################

###  http://www.w3.org/2004/02/skos/core#inScheme
<http://www.w3.org/2004/02/skos/core#inScheme> rdf:type owl:ObjectProperty .


###  https://w3id.org/transmodel/commons#in
<https://w3id.org/transmodel/commons#in> rdf:type owl:ObjectProperty .


###  https://w3id.org/transmodel/facilities#OBJECTPROPERTIESTOREVIEW
:OBJECTPROPERTIESTOREVIEW rdf:type owl:ObjectProperty .


###  https://w3id.org/transmodel/facilities#accessedBy
:accessedBy rdf:type owl:ObjectProperty ;
            rdfs:comment "This property sets the relationship between Site and Entrance"@en ;
            rdfs:label "accessed by"@en .


###  https://w3id.org/transmodel/facilities#accessibilityAssessment
:accessibilityAssessment rdf:type owl:ObjectProperty ;
                         rdfs:subPropertyOf owl:topObjectProperty ;
                         rdfs:range :AccessibilityAssessment ;
                         rdfs:comment "TODO: Determine whether this should be moved to another module if the concept AccessibilityAssessment is moved as well"@en ,
                                      "This property is used to relate a site element, a facility, etc., with a specific accessibility assessment. In some of the UML models of Transmodel this property is name as characerisedBy"@en ;
                         rdfs:label "accessibility assessment"@en .


###  https://w3id.org/transmodel/facilities#accessibilityLimitation
:accessibilityLimitation rdf:type owl:ObjectProperty ;
                         rdfs:subPropertyOf :OBJECTPROPERTIESTOREVIEW ;
                         rdfs:domain :Facility ;
                         rdfs:label "accessibilityLimitation"@en .


###  https://w3id.org/transmodel/facilities#accommodationFacility
:accommodationFacility rdf:type owl:ObjectProperty ;
                       rdfs:subPropertyOf :facilityType ;
                       rdfs:domain :Accommodation ;
                       rdfs:range [ owl:intersectionOf ( <http://www.w3.org/2004/02/skos/core#Concept>
                                                         [ rdf:type owl:Restriction ;
                                                           owl:onProperty <http://www.w3.org/2004/02/skos/core#inScheme> ;
                                                           owl:hasValue <https://w3id.org/transmodel/kos/facilities/FacilityType>
                                                         ]
                                                       ) ;
                                    rdf:type owl:Class
                                  ] ;
                       rdfs:comment "TODO: the range of this property may be further restricted to those SKOS concepts that also comply with skos:broader tmkosfacility:FacilityType/AccomodationFacilityType"@en ,
                                    "This property restricts the type of facility to one specific for accommodation from the SKOS codelist for types of facilities, including, for example, values like seating, sleeper, couchette, special seating, reclining seats, standing, etc."@en ;
                       rdfs:label "accommodation facility"@en .


###  https://w3id.org/transmodel/facilities#accomodation
:accomodation rdf:type owl:ObjectProperty ;
              rdfs:subPropertyOf :OBJECTPROPERTIESTOREVIEW ;
              rdfs:domain <https://w3id.org/transmodel/journeys#Service> ;
              rdfs:label "accomodation"@en .


###  https://w3id.org/transmodel/facilities#activateEquipment
:activateEquipment rdf:type owl:ObjectProperty ;
                   rdfs:subPropertyOf :OBJECTPROPERTIESTOREVIEW ;
                   rdfs:domain :Passenger ;
                   rdfs:range :Equipment ;
                   rdfs:label "activateEquipment"@en .


###  https://w3id.org/transmodel/facilities#activationAssignment
:activationAssignment rdf:type owl:ObjectProperty ;
                      rdfs:subPropertyOf :OBJECTPROPERTIESTOREVIEW ;
                      rdfs:label "activationAssignment"@en .


###  https://w3id.org/transmodel/facilities#availableAt
:availableAt rdf:type owl:ObjectProperty ;
             rdfs:domain :SiteFacilitySet ;
             rdfs:range :Site ;
             rdfs:comment "TODO: Check whether this property is also applicable to other things beyond Site Facility Sets"@en ,
                          "This property relates a Site Facility Set with a Site"@en ;
             rdfs:label "available at"@en .


###  https://w3id.org/transmodel/facilities#boardingPermission
:boardingPermission rdf:type owl:ObjectProperty ;
                    rdfs:subPropertyOf :facilityType ;
                    rdfs:domain :OnboardStay ;
                    rdfs:range [ owl:intersectionOf ( <http://www.w3.org/2004/02/skos/core#Concept>
                                                      [ rdf:type owl:Restriction ;
                                                        owl:onProperty <http://www.w3.org/2004/02/skos/core#inScheme> ;
                                                        owl:hasValue <https://w3id.org/transmodel/kos/facilities/FacilityType>
                                                      ]
                                                    ) ;
                                 rdf:type owl:Class
                               ] ;
                    rdfs:comment "TODO: the range of this property may be further restricted to those SKOS concepts that also comply with skos:broader tmkosfacility:FacilityType/BoardingPermissionType"@en ,
                                 "This property describes the types of boarding permissions allowed for an Onboard Stay from the SKOS codelist for types of facilities, including normal, early boarding, late alighting, etc."@en ;
                    rdfs:label "boarding permission"@en .


###  https://w3id.org/transmodel/facilities#checkConstraint
:checkConstraint rdf:type owl:ObjectProperty ;
                 rdfs:subPropertyOf :OBJECTPROPERTIESTOREVIEW ;
                 rdfs:domain :SiteComponent ;
                 rdfs:range :Constraint ;
                 rdfs:label "siteComponentCheckConstraint"@en .


###  https://w3id.org/transmodel/facilities#comprises
:comprises rdf:type owl:ObjectProperty ;
           rdfs:comment "General property for all types of containment and aggregation"@en ;
           rdfs:label "comprises"@en .


###  https://w3id.org/transmodel/facilities#comprisesEquipment
:comprisesEquipment rdf:type owl:ObjectProperty ;
                    rdfs:subPropertyOf :comprises ;
                    rdfs:domain :FacilitySet ;
                    rdfs:range :Equipment ;
                    rdfs:comment "TODO: Check carefully whether the range should be Equipment or, instead, something more general like Facility, since the differentiation between Facility and Equipment is sometimes unclear"@en ,
                                 """This property is used to aggregate other types of facilities from a Facility Set, normally focused on those that are user defined and not from the predefined list.
In the Transmodel UML model this is represented as TypeOfEquipment, and in the Netex implementation the term otherFacilities is used."""@en ;
                    rdfs:label "comprises equipment"@en .


###  https://w3id.org/transmodel/facilities#comprisesFacility
:comprisesFacility rdf:type owl:ObjectProperty ;
                   rdfs:subPropertyOf :comprises ;
                   rdfs:domain :FacilitySet ;
                   rdfs:range :Facility ;
                   rdfs:comment """This property is used to aggregate all the facilities that a facility set contains
In Netex, this is expressed with the element TypeOfFacilityRef, which is used to refer to facilities, and in the Transmodel UML ontology this is simply expressed as 'facility'"""@en ;
                   rdfs:label "comprises facility"@en .


###  https://w3id.org/transmodel/facilities#concernedBy
:concernedBy rdf:type owl:ObjectProperty ;
             rdfs:range :FacilitySet ;
             rdfs:comment "This property allows connecting any object with a Facility Set"@en ;
             rdfs:label "concerned by"@en .


###  https://w3id.org/transmodel/facilities#containing
:containing rdf:type owl:ObjectProperty ;
            rdfs:comment "This property allows specifying that a Stop contains Quays"@en ;
            rdfs:label "containing"@en .


###  https://w3id.org/transmodel/facilities#couchetteFacility
:couchetteFacility rdf:type owl:ObjectProperty ;
                   rdfs:subPropertyOf :facilityType ;
                   rdfs:domain :Accommodation ;
                   rdfs:range [ owl:intersectionOf ( <http://www.w3.org/2004/02/skos/core#Concept>
                                                     [ rdf:type owl:Restriction ;
                                                       owl:onProperty <http://www.w3.org/2004/02/skos/core#inScheme> ;
                                                       owl:hasValue <https://w3id.org/transmodel/kos/facilities/FacilityType>
                                                     ]
                                                   ) ;
                                rdf:type owl:Class
                              ] ;
                   rdfs:comment "TODO: the range of this property may be further restricted to those SKOS concepts that also comply with skos:broader tmkosfacility:FacilityType/CouchetteFacilityType"@en ,
                                "This property restricts the type of facility to one specific for couchette from the SKOS codelist for types of facilities, including, for example, values like T2, T3, C1, C2, etc."@en ;
                   rdfs:label "couchette facility"@en .


###  https://w3id.org/transmodel/facilities#determining
:determining rdf:type owl:ObjectProperty ;
             rdfs:domain :AccessibilityAssessment ;
             rdfs:range :AccessibilityLimitation ;
             rdfs:comment "This property sets the relationship between Accessibility Assessment and Accessibility Limitation"@en ;
             rdfs:label "determining"@en .


###  https://w3id.org/transmodel/facilities#displayAssignment
:displayAssignment rdf:type owl:ObjectProperty ;
                   rdfs:subPropertyOf :OBJECTPROPERTIESTOREVIEW ;
                   rdfs:domain :JourneyPattern ;
                   rdfs:comment "The assignment of one ScheduledStopPoint and one JourneyPattern to a PassengerInformationEquipment specifying that information on the ScheduledStopPoint and the JourneyPattern will be provided (e.g. displayed, printed)"@en ;
                   rdfs:label "displayAssignment"@en .


###  https://w3id.org/transmodel/facilities#equipmentType
:equipmentType rdf:type owl:ObjectProperty ;
               rdfs:subPropertyOf owl:topObjectProperty ;
               rdfs:domain :Equipment ;
               rdfs:range [ owl:intersectionOf ( <http://www.w3.org/2004/02/skos/core#Concept>
                                                 [ rdf:type owl:Restriction ;
                                                   owl:onProperty <http://www.w3.org/2004/02/skos/core#inScheme> ;
                                                   owl:hasValue <https://w3id.org/transmodel/kos/facilities/EquipmentType>
                                                 ]
                                               ) ;
                            rdf:type owl:Class
                          ] ;
               rdfs:comment "This property is used to link an equipment with the types of equipments available in the SKOS concept scheme of types of equipments"@en ;
               rdfs:label "equipment Type"@en .


###  https://w3id.org/transmodel/facilities#equippedWith
:equippedWith rdf:type owl:ObjectProperty ;
              rdfs:domain :EquipmentPlace ;
              rdfs:range :Equipment ;
              rdfs:comment "TODO: relate it to a more general property for containment and partOf"@en ,
                           "This property is used to define the equipments that are available in an equipment place"@en ;
              rdfs:label "equipped With"@en .


###  https://w3id.org/transmodel/facilities#facilityRequirement
:facilityRequirement rdf:type owl:ObjectProperty ;
                     rdfs:subPropertyOf :OBJECTPROPERTIESTOREVIEW ;
                     rdfs:domain :Vehicle ;
                     rdfs:range :Facility ;
                     rdfs:comment "A classification of public transport Vehicles according to the facilities available on the Vehicle"@en ;
                     rdfs:label "facilityRequirement"@en .


###  https://w3id.org/transmodel/facilities#facilitySet
:facilitySet rdf:type owl:ObjectProperty ;
             rdfs:subPropertyOf :OBJECTPROPERTIESTOREVIEW ;
             rdfs:comment "Set of Facilities available for a ServiceJourney or a JourneyPart. The set may be available only for a specific VehicleType within the service (e.g. carriage equipped with low floor)"@en ;
             rdfs:label "facilitySet"@en .


###  https://w3id.org/transmodel/facilities#facilityType
:facilityType rdf:type owl:ObjectProperty ;
              rdfs:domain :Facility ;
              rdfs:range [ owl:intersectionOf ( <http://www.w3.org/2004/02/skos/core#Concept>
                                                [ rdf:type owl:Restriction ;
                                                  owl:onProperty <http://www.w3.org/2004/02/skos/core#inScheme> ;
                                                  owl:hasValue <https://w3id.org/transmodel/kos/facilities/FacilityType>
                                                ]
                                              ) ;
                           rdf:type owl:Class
                         ] ;
              rdfs:comment "This property is used to link a facility with the types of facilities available in the SKOS concept scheme of types of facilities"@en ,
                           "facility type"@en .


###  https://w3id.org/transmodel/facilities#fareClass
:fareClass rdf:type owl:ObjectProperty ;
           rdfs:subPropertyOf :facilityType ;
           rdfs:domain :ServiceFacilitySet ;
           rdfs:range [ owl:intersectionOf ( <http://www.w3.org/2004/02/skos/core#Concept>
                                             [ rdf:type owl:Restriction ;
                                               owl:onProperty <http://www.w3.org/2004/02/skos/core#inScheme> ;
                                               owl:hasValue <https://w3id.org/transmodel/kos/facilities/FacilityType>
                                             ]
                                           ) ;
                        rdf:type owl:Class
                      ] ;
           rdfs:comment "TODO: create the list of allowed values for fare classes, and check whether including it as a facility type, as included in the TransModel model"@en ,
                        "This property relates an Onboard Stay or an Accommodation, among others, with a class of fares, whose allowed values are defined in the TransModel Common Facility Values (Figure 290, page 454)"@en ;
           rdfs:label "fare class"@en .


###  https://w3id.org/transmodel/facilities#isUsedBy
:isUsedBy rdf:type owl:ObjectProperty ;
          rdfs:subPropertyOf :OBJECTPROPERTIESTOREVIEW ;
          rdfs:domain :Facility ;
          rdfs:range :Passenger ;
          rdfs:label "isUsedBy"@en .


###  https://w3id.org/transmodel/facilities#locatedIn
:locatedIn rdf:type owl:ObjectProperty ;
           rdfs:domain :Equipment ;
           rdfs:range :EquipmentPlace ;
           rdfs:comment "TODO: find a more general property (probably similar to contains/containedIn) and think about whether it should be replaced by this more general property, or at least created as a subProperty of that one."@en ,
                        "This property is used to relate an equipment with the equipment place where it is located"@en ;
           rdfs:label "located in"@en .


###  https://w3id.org/transmodel/facilities#noticeAssignment
:noticeAssignment rdf:type owl:ObjectProperty ;
                  rdfs:subPropertyOf :OBJECTPROPERTIESTOREVIEW ;
                  rdfs:domain :JourneyPattern ;
                  rdfs:range :Notice ;
                  rdfs:comment "The assignment of a Notice showing an exception in a JourneyPattern, a CommonSection or a VehicleJourney, possibly specifying at which PointInJourneyPattern the validity of the Notice starts and ends respectively"@en ;
                  rdfs:label "noticeAssignment"@en .


###  https://w3id.org/transmodel/facilities#position
:position rdf:type owl:ObjectProperty ;
          rdfs:domain [ rdf:type owl:Class ;
                        owl:unionOf ( :EquipmentPlace
                                      :PlaceEquipment
                                    )
                      ] ;
          rdfs:range :EquipmentPosition ;
          rdfs:comment "This property is used to relate an equipment place (a collection of equipments) or a specific place equipment with the different equipment positions that they may have"@en ;
          rdfs:label "position"@en .


###  https://w3id.org/transmodel/facilities#presentAt
:presentAt rdf:type owl:ObjectProperty ;
           rdfs:domain :ServiceFacilitySet ;
           rdfs:range :VehicleType ;
           rdfs:comment "This property relates a Service Facility Set with a Vehicle Type, indicating that the set of service facilities comprised by the set are provided at that type of vehicle"@en ;
           rdfs:label "present at"@en .


###  https://w3id.org/transmodel/facilities#providedBy
:providedBy rdf:type owl:ObjectProperty ;
            rdfs:subPropertyOf owl:topObjectProperty ;
            rdfs:domain :FacilitySet ;
            rdfs:comment """TODO: Add org:Organization as range for this property
TODO: Check whether the domain should be generalised (applicable not only to facility set but also to facility, site, equipment, etc.)"""@es ,
                         """This property is used to refer to the provider of a facility set
In the TransModel UML model and in the Netex implementation this is expressed as ProvidedByRef"""@es ;
            rdfs:label "provided by"@es .


###  https://w3id.org/transmodel/facilities#showerFacility
:showerFacility rdf:type owl:ObjectProperty ;
                rdfs:subPropertyOf :facilityType ;
                rdfs:domain :Accommodation ;
                rdfs:range [ owl:intersectionOf ( <http://www.w3.org/2004/02/skos/core#Concept>
                                                  [ rdf:type owl:Restriction ;
                                                    owl:onProperty <http://www.w3.org/2004/02/skos/core#inScheme> ;
                                                    owl:hasValue <https://w3id.org/transmodel/kos/facilities/FacilityType>
                                                  ]
                                                ) ;
                             rdf:type owl:Class
                           ] ;
                rdfs:comment "TODO: the range of this property may be further restricted to those SKOS concepts that also comply with skos:broader tmkosfacility:FacilityType/XXX, where XXX refers to the shower facilities"@en ,
                             "This property restricts the type of facility to one specific for shower from the SKOS codelist for types of facilities. However, there is no specific part of the codelist reserved yet for shower facilities."@en ;
                rdfs:label "shower facility"@en .


###  https://w3id.org/transmodel/facilities#stopPlaceComponent
:stopPlaceComponent rdf:type owl:ObjectProperty ;
                    rdfs:subPropertyOf :OBJECTPROPERTIESTOREVIEW ;
                    rdfs:range :StopPlaceComponent ;
                    rdfs:label "stopPlaceComponent"@en .


###  https://w3id.org/transmodel/facilities#stopPlaceEntrance
:stopPlaceEntrance rdf:type owl:ObjectProperty ;
                   rdfs:subPropertyOf :OBJECTPROPERTIESTOREVIEW ;
                   rdfs:range :AccessEquipment ;
                   rdfs:comment "A physical entrance or exit to/from a StopPlace for a Passenger. May be a door, barrier, gate other recognizable point of access"@en ,
                                "stopPlaceEntrance"@en .


###  https://w3id.org/transmodel/facilities#subplaceOf
:subplaceOf rdf:type owl:ObjectProperty ;
            rdfs:domain :StopPlace ;
            rdfs:range :StopPlace ;
            rdfs:comment "A property connecting one Stop Place to another Stop Place to describe nested Stop Places (e.g. a metro station in a train station)."@en ;
            rdfs:label "subplace of"@en .


###  https://w3id.org/transmodel/facilities#toiletFacility
:toiletFacility rdf:type owl:ObjectProperty ;
                rdfs:subPropertyOf :facilityType ;
                rdfs:domain :Accommodation ;
                rdfs:range [ owl:intersectionOf ( <http://www.w3.org/2004/02/skos/core#Concept>
                                                  [ rdf:type owl:Restriction ;
                                                    owl:onProperty <http://www.w3.org/2004/02/skos/core#inScheme> ;
                                                    owl:hasValue <https://w3id.org/transmodel/kos/facilities/FacilityType>
                                                  ]
                                                ) ;
                             rdf:type owl:Class
                           ] ;
                rdfs:comment "TODO: the range of this property may be further restricted to those SKOS concepts that also comply with skos:broader tmkosfacility:FacilityType/XXX, where XXX refers to the toilet facilities"@en ,
                             "This property restricts the type of facility to one specific for toilets from the SKOS codelist for types of facilities. However, there is no specific part of the codelist reserved yet for toilet facilities (also known as sanitary facilities)."@en ;
                rdfs:label "toilet facility"@en .


###  https://w3id.org/transmodel/facilities#typeOfAccessFeature
:typeOfAccessFeature rdf:type owl:ObjectProperty ;
                     rdfs:subPropertyOf :OBJECTPROPERTIESTOREVIEW ;
                     rdfs:domain :ConstraintOfAccess .


###  https://w3id.org/transmodel/facilities#typeOfAccessibilityTools
:typeOfAccessibilityTools rdf:type owl:ObjectProperty ;
                          rdfs:subPropertyOf :OBJECTPROPERTIESTOREVIEW ;
                          rdfs:domain :AssistanceService ;
                          rdfs:label "typeOfAccessibilityTools"@en .


###  https://w3id.org/transmodel/facilities#typeOfCateringService
:typeOfCateringService rdf:type owl:ObjectProperty ;
                       rdfs:subPropertyOf :OBJECTPROPERTIESTOREVIEW ;
                       rdfs:domain :CateringService ;
                       rdfs:label "typeOfCateringService"@en .


###  https://w3id.org/transmodel/facilities#typeOfCheckConstraint
:typeOfCheckConstraint rdf:type owl:ObjectProperty ;
                       rdfs:subPropertyOf :OBJECTPROPERTIESTOREVIEW ;
                       rdfs:domain :Constraint ;
                       rdfs:label "typeOfCheckConstraint"@en .


###  https://w3id.org/transmodel/facilities#typeOfCongestion
:typeOfCongestion rdf:type owl:ObjectProperty ;
                  rdfs:subPropertyOf :OBJECTPROPERTIESTOREVIEW ;
                  rdfs:label "typeOfCongestion"@en .


###  https://w3id.org/transmodel/facilities#typeOfCycleEquipment
:typeOfCycleEquipment rdf:type owl:ObjectProperty ;
                      rdfs:subPropertyOf :OBJECTPROPERTIESTOREVIEW ;
                      rdfs:domain :CycleOperatingEquipment ;
                      rdfs:label "typeOfCycleStorageEquipment" .


###  https://w3id.org/transmodel/facilities#typeOfEmergencyService
:typeOfEmergencyService rdf:type owl:ObjectProperty ;
                        rdfs:subPropertyOf :OBJECTPROPERTIESTOREVIEW ;
                        rdfs:domain :EmergencyService ;
                        rdfs:label "typeOfEmergencyService"@en .


###  https://w3id.org/transmodel/facilities#typeOfEntranceEquipment
:typeOfEntranceEquipment rdf:type owl:ObjectProperty ;
                         rdfs:subPropertyOf :OBJECTPROPERTIESTOREVIEW ;
                         rdfs:domain :EntranceEquipment ;
                         rdfs:comment "Classification of the Entrance Equipment"@en ;
                         rdfs:label "typeOfEntranceEquipment"@en .


###  https://w3id.org/transmodel/facilities#typeOfGenderLimitation
:typeOfGenderLimitation rdf:type owl:ObjectProperty ;
                        rdfs:subPropertyOf :OBJECTPROPERTIESTOREVIEW ;
                        rdfs:domain :SanitaryEquipment ;
                        rdfs:label "typeOfGenderLimitation"@en .


###  https://w3id.org/transmodel/facilities#typeOfHandrail
:typeOfHandrail rdf:type owl:ObjectProperty ;
                rdfs:subPropertyOf :OBJECTPROPERTIESTOREVIEW ;
                rdfs:domain :StairEquipment ;
                rdfs:comment "types of handrails" ;
                rdfs:label "typeOfHandrail"@en .


###  https://w3id.org/transmodel/facilities#typeOfPassengerInformationDesk
:typeOfPassengerInformationDesk rdf:type owl:ObjectProperty ;
                                rdfs:subPropertyOf :OBJECTPROPERTIESTOREVIEW ;
                                rdfs:domain :PassengerInformationEquipment ;
                                rdfs:comment "The relationship between the PassengerInformationDesk with the typeOfInformationDesk"@en ;
                                rdfs:label "typeOfPassengerInformationDesk"@en .


###  https://w3id.org/transmodel/facilities#typeOfPlaceAccessStair
:typeOfPlaceAccessStair rdf:type owl:ObjectProperty ;
                        rdfs:subPropertyOf :OBJECTPROPERTIESTOREVIEW ;
                        rdfs:domain :StairEquipment ;
                        rdfs:label "typeOfPlaceAccessStairs"@en .


###  https://w3id.org/transmodel/facilities#typeOfSanitaryEquipment
:typeOfSanitaryEquipment rdf:type owl:ObjectProperty ;
                         rdfs:subPropertyOf :OBJECTPROPERTIESTOREVIEW ;
                         rdfs:range :SanitaryEquipment ;
                         rdfs:label "typeOfSanitaryEquipment"@en .


###  https://w3id.org/transmodel/facilities#typeOfVehicle
:typeOfVehicle rdf:type owl:ObjectProperty ;
               rdfs:subPropertyOf :OBJECTPROPERTIESTOREVIEW ;
               rdfs:domain :Vehicle ;
               rdfs:range :VehicleType ;
               rdfs:label "typeOfVehicle"@en .


###  https://w3id.org/transmodel/facilities#typeOfWaitingRoom
:typeOfWaitingRoom rdf:type owl:ObjectProperty ;
                   rdfs:subPropertyOf :OBJECTPROPERTIESTOREVIEW ;
                   rdfs:domain :WaitingRoomEquipment ;
                   rdfs:label "typeOfWaitingRoomEquipment"@en .


###  https://w3id.org/transmodel/facilities#userNeedSuitability
:userNeedSuitability rdf:type owl:ObjectProperty ;
                     rdfs:subPropertyOf :OBJECTPROPERTIESTOREVIEW ;
                     rdfs:domain :UserNeed ;
                     rdfs:range :Suitability ;
                     rdfs:label "userNeedSuitability"@en .


###  https://w3id.org/transmodel/facilities#validityConditionDefines
:validityConditionDefines rdf:type owl:ObjectProperty ;
                          rdfs:subPropertyOf :OBJECTPROPERTIESTOREVIEW ;
                          rdfs:domain :ValidityCondition ;
                          rdfs:range :ValidityTrigger ;
                          rdfs:label "validityConditionDefines"@en .


###  https://w3id.org/transmodel/facilities#wheelchairAccess
:wheelchairAccess rdf:type owl:ObjectProperty ;
                  rdfs:domain :AccessibilityLimitation ;
                  rdfs:range [ owl:intersectionOf ( <http://www.w3.org/2004/02/skos/core#Concept>
                                                    [ rdf:type owl:Restriction ;
                                                      owl:onProperty <http://www.w3.org/2004/02/skos/core#inScheme> ;
                                                      owl:hasValue <https://w3id.org/transmodel/kos/journeys/mobility-limitation>
                                                    ]
                                                  ) ;
                               rdf:type owl:Class
                             ] ;
                  rdfs:comment "This property sets the relationaship between Accessibility Limitation and the kos wheelchair-access"@en ;
                  rdfs:label "wheelchair Access"@en .


###  https://w3id.org/transmodel/journeys#hasAServiceJourneyPattern
<https://w3id.org/transmodel/journeys#hasAServiceJourneyPattern> rdf:type owl:ObjectProperty ;
                                                                 rdfs:subPropertyOf :OBJECTPROPERTIESTOREVIEW ;
                                                                 rdfs:domain <https://w3id.org/transmodel/journeys#Service> .


###  https://w3id.org/transmodel/journeys#makesAServiceJourney
<https://w3id.org/transmodel/journeys#makesAServiceJourney> rdf:type owl:ObjectProperty ;
                                                            rdfs:subPropertyOf :OBJECTPROPERTIESTOREVIEW ;
                                                            rdfs:range <https://w3id.org/transmodel/journeys#Service> .


#################################################################
#    Data properties
#################################################################

###  https://w3id.org/transmodel/commons#borderCrossing
<https://w3id.org/transmodel/commons#borderCrossing> rdf:type owl:DatatypeProperty .


###  https://w3id.org/transmodel/facilities#DATAPROPERTIESTOREVIEW
:DATAPROPERTIESTOREVIEW rdf:type owl:DatatypeProperty .


###  https://w3id.org/transmodel/facilities#accessDimensions
:accessDimensions rdf:type owl:DatatypeProperty ;
                  rdfs:subPropertyOf :DATAPROPERTIESTOREVIEW ;
                  rdfs:domain :WheelchairVehicleEquipment ;
                  rdfs:range rdfs:Literal .


###  https://w3id.org/transmodel/facilities#activatedEquipment
:activatedEquipment rdf:type owl:DatatypeProperty ;
                    rdfs:subPropertyOf :DATAPROPERTIESTOREVIEW ;
                    rdfs:domain :Facility ;
                    rdfs:range xsd:boolean ;
                    rdfs:label "activatedEquipment"@en .


###  https://w3id.org/transmodel/facilities#constraintThroughput
:constraintThroughput rdf:type owl:DatatypeProperty ;
                      rdfs:subPropertyOf :DATAPROPERTIESTOREVIEW ;
                      rdfs:domain :ConstraintThroughput ;
                      rdfs:range xsd:integer ;
                      rdfs:label "constraintThroughtput"@en .


###  https://w3id.org/transmodel/facilities#duration
:duration rdf:type owl:DatatypeProperty ;
          rdfs:domain :OnboardStay ;
          rdfs:range xsd:duration ;
          rdfs:comment "This property relates an Onboard Stay with a duration"@en ;
          rdfs:label "duration"@en .


###  https://w3id.org/transmodel/facilities#facilityLocation
:facilityLocation rdf:type owl:DatatypeProperty ;
                  rdfs:subPropertyOf :DATAPROPERTIESTOREVIEW ;
                  rdfs:domain :Facility ;
                  rdfs:label "facilityLocation" .


###  https://w3id.org/transmodel/facilities#fixed
:fixed rdf:type owl:DatatypeProperty ;
       rdfs:domain :Equipment ;
       rdfs:range xsd:boolean ;
       rdfs:comment "This property is used to determine whether an equipment is fixed in a place or not."@en ;
       rdfs:label "fixed"@en .


###  https://w3id.org/transmodel/facilities#freeToUse
:freeToUse rdf:type owl:DatatypeProperty ;
           rdfs:subPropertyOf :DATAPROPERTIESTOREVIEW ;
           rdfs:domain :LocalService ;
           rdfs:range xsd:boolean ;
           rdfs:comment "Characteristic of a Service that is free to use it"@en ;
           rdfs:label "freeToUse"@en .


###  https://w3id.org/transmodel/facilities#outOfService
:outOfService rdf:type owl:DatatypeProperty ;
              rdfs:domain :Equipment ;
              rdfs:range xsd:boolean ;
              rdfs:comment "This property allows specifying whether the equipment is out of service or not"@en ;
              rdfs:label "out of service"@en .


###  https://w3id.org/transmodel/facilities#siteComponentTimePenalty
:siteComponentTimePenalty rdf:type owl:DatatypeProperty ;
                          rdfs:subPropertyOf :DATAPROPERTIESTOREVIEW ;
                          rdfs:domain :ConstraintDelay ;
                          rdfs:range xsd:dateTime ;
                          rdfs:label "constraintDelayInterval"@en .


###  https://w3id.org/transmodel/facilities#wheelchairAreas
:wheelchairAreas rdf:type owl:DatatypeProperty ;
                 rdfs:subPropertyOf :DATAPROPERTIESTOREVIEW ;
                 rdfs:domain :WheelchairVehicleEquipment ;
                 rdfs:range xsd:integer .


#################################################################
#    Classes
#################################################################

###  http://www.w3.org/2004/02/skos/core#Concept
<http://www.w3.org/2004/02/skos/core#Concept> rdf:type owl:Class .


###  http://www.w3.org/2004/02/skos/core#ConceptScheme
<http://www.w3.org/2004/02/skos/core#ConceptScheme> rdf:type owl:Class .


###  https://w3id.org/transmodel/facilities#AccessAreaDimensions
:AccessAreaDimensions rdf:type owl:Class ;
                      rdfs:subClassOf :VehicleAccessEquipment ;
                      rdfs:comment "Specialisation of VehicleAccessEquipment dedicated to VehicleAccessAreaDimmension"@en ,
                                   "TODO: Check if this has to be maintained, as it is not present in the Equipment Overview Physical Model of Transmodel (figure 247)"@en ;
                      rdfs:label "VehicleAccessAreaDimension"@en .


###  https://w3id.org/transmodel/facilities#AccessEquipment
:AccessEquipment rdf:type owl:Class ;
                 rdfs:subClassOf :PlaceEquipment ;
                 rdfs:comment "Specialisation of Place Equipment dedicated to access (e.g. lifts, entrances, stairs, ramps, etc.)"@en ;
                 rdfs:label "Access Equipment"@en .


###  https://w3id.org/transmodel/facilities#AccessSpace
:AccessSpace rdf:type owl:Class ;
             owl:equivalentClass :PassengerArea ;
             rdfs:subClassOf :THINGSTOREVIEW ;
             rdfs:label "AccessSpace"@en .


###  https://w3id.org/transmodel/facilities#AccessibilityAssessment
:AccessibilityAssessment rdf:type owl:Class ;
                         rdfs:comment "The accessibility characteristics of an Entity (facility)  used by Passenger such as a Stop Place or a Stop Place Component. Described by AccessibilityLimitations and/or a set of Suitabilities"@en ;
                         rdfs:label "Accessibility Assessment"@en .


###  https://w3id.org/transmodel/facilities#AccessibilityLimitation
:AccessibilityLimitation rdf:type owl:Class ;
                         rdfs:subClassOf [ rdf:type owl:Restriction ;
                                           owl:onProperty :determining ;
                                           owl:allValuesFrom :AccessibilityLimitation
                                         ] ;
                         rdfs:comment """A categorisation of the accessibility characteristics of a Site, e.g. a Stop Place or a Stop Place Component to indicate its usability by passengers with specific needs, for example, those needing wheelchair access, step-free access or wanting to avoid confined spaces such as lifts. 
A small number of well-defined categories are used that are chosen to allow the consistent capture of data and the efficient computation of routes for different classes of user."""@en ;
                         rdfs:label "Accessibility Limitation"@en .


###  https://w3id.org/transmodel/facilities#Accommodation
:Accommodation rdf:type owl:Class ;
               rdfs:subClassOf :Facility ,
                               [ rdf:type owl:Restriction ;
                                 owl:onProperty :accommodationFacility ;
                                 owl:maxQualifiedCardinality "1"^^xsd:nonNegativeInteger ;
                                 owl:onClass [ owl:intersectionOf ( <http://www.w3.org/2004/02/skos/core#Concept>
                                                                    [ rdf:type owl:Restriction ;
                                                                      owl:onProperty <http://www.w3.org/2004/02/skos/core#inScheme> ;
                                                                      owl:hasValue <https://w3id.org/transmodel/kos/facilities/FacilityType>
                                                                    ]
                                                                  ) ;
                                               rdf:type owl:Class
                                             ]
                               ] ,
                               [ rdf:type owl:Restriction ;
                                 owl:onProperty :couchetteFacility ;
                                 owl:maxQualifiedCardinality "1"^^xsd:nonNegativeInteger ;
                                 owl:onClass [ owl:intersectionOf ( <http://www.w3.org/2004/02/skos/core#Concept>
                                                                    [ rdf:type owl:Restriction ;
                                                                      owl:onProperty <http://www.w3.org/2004/02/skos/core#inScheme> ;
                                                                      owl:hasValue <https://w3id.org/transmodel/kos/facilities/FacilityType>
                                                                    ]
                                                                  ) ;
                                               rdf:type owl:Class
                                             ]
                               ] ,
                               [ rdf:type owl:Restriction ;
                                 owl:onProperty :fareClass ;
                                 owl:maxQualifiedCardinality "1"^^xsd:nonNegativeInteger ;
                                 owl:onClass [ owl:intersectionOf ( <http://www.w3.org/2004/02/skos/core#Concept>
                                                                    [ rdf:type owl:Restriction ;
                                                                      owl:onProperty <http://www.w3.org/2004/02/skos/core#inScheme> ;
                                                                      owl:hasValue <https://w3id.org/transmodel/kos/facilities/FacilityType>
                                                                    ]
                                                                  ) ;
                                               rdf:type owl:Class
                                             ]
                               ] ,
                               [ rdf:type owl:Restriction ;
                                 owl:onProperty :showerFacility ;
                                 owl:maxQualifiedCardinality "1"^^xsd:nonNegativeInteger ;
                                 owl:onClass [ owl:intersectionOf ( <http://www.w3.org/2004/02/skos/core#Concept>
                                                                    [ rdf:type owl:Restriction ;
                                                                      owl:onProperty <http://www.w3.org/2004/02/skos/core#inScheme> ;
                                                                      owl:hasValue <https://w3id.org/transmodel/kos/facilities/FacilityType>
                                                                    ]
                                                                  ) ;
                                               rdf:type owl:Class
                                             ]
                               ] ,
                               [ rdf:type owl:Restriction ;
                                 owl:onProperty :toiletFacility ;
                                 owl:maxQualifiedCardinality "1"^^xsd:nonNegativeInteger ;
                                 owl:onClass [ owl:intersectionOf ( <http://www.w3.org/2004/02/skos/core#Concept>
                                                                    [ rdf:type owl:Restriction ;
                                                                      owl:onProperty <http://www.w3.org/2004/02/skos/core#inScheme> ;
                                                                      owl:hasValue <https://w3id.org/transmodel/kos/facilities/FacilityType>
                                                                    ]
                                                                  ) ;
                                               rdf:type owl:Class
                                             ]
                               ] ;
               rdfs:comment "This is a subclass of Service Facility Set to refer to types of accommodations, according to the Facility Conceptual Model (figure 287, page 450) of TransModel"@en ;
               rdfs:label "Accommodation"@en .


###  https://w3id.org/transmodel/facilities#ActivationLink
:ActivationLink rdf:type owl:Class ;
                rdfs:subClassOf :THINGSTOREVIEW ;
                rdfs:comment "A Link where a control process is acivated when a vehicle passes it."@en ;
                rdfs:label "ActivationLink"@en .


###  https://w3id.org/transmodel/facilities#ActivationPoint
:ActivationPoint rdf:type owl:Class ;
                 rdfs:subClassOf <https://w3id.org/transmodel/journeys#Point> ;
                 rdfs:comment "A Point where a control process is activated when a vehicle passes it. equipment may be needed for activation."@en ;
                 rdfs:label "ActivationPoint"@en .


###  https://w3id.org/transmodel/facilities#AssistanceForDissabledUsers
:AssistanceForDissabledUsers rdf:type owl:Class ;
                             rdfs:subClassOf :AssistanceService ;
                             rdfs:comment "Assistance Services for dissabled users of the Public Transport Network"@en ,
                                          "TODO: Check if this has to be maintained, as it is not present in the Equipment Overview Physical Model of Transmodel (figure 247)"@en ;
                             rdfs:label "AssistanceForDissabledUsers"@en .


###  https://w3id.org/transmodel/facilities#AssistanceService
:AssistanceService rdf:type owl:Class ;
                   rdfs:subClassOf :LocalService ;
                   rdfs:comment "Specialisation of LocalService for Assistance providing information like language, accessibility trained staff, etc."@en ;
                   rdfs:label "AssistanceService"@en .


###  https://w3id.org/transmodel/facilities#BabyChange
:BabyChange rdf:type owl:Class ;
            rdfs:subClassOf :SanitaryEquipment ;
            rdfs:comment "TODO: Check if this has to be maintained, as it is not present in the Equipment Overview Physical Model of Transmodel (figure 247)"@en .


###  https://w3id.org/transmodel/facilities#BookingOffice
:BookingOffice rdf:type owl:Class ;
               rdfs:subClassOf :CustomerService ;
               rdfs:comment "A specialisation of Customer Services for booking services"@en ,
                            "TODO: Check if this has to be maintained, as it is not present in the Equipment Overview Physical Model of Transmodel (figure 247)"@en ;
               rdfs:label "BookingOffice"@en .


###  https://w3id.org/transmodel/facilities#CateringService
:CateringService rdf:type owl:Class ;
                 rdfs:subClassOf :CommercialService ;
                 rdfs:comment "Specialisation of LocalService for CateringService"@en ;
                 rdfs:label "CateringService"@en .


###  https://w3id.org/transmodel/facilities#CheckIn
:CheckIn rdf:type owl:Class ;
         rdfs:subClassOf :EquipmentPlace ;
         rdfs:comment "One specialisation of SiteComponent for Check in services"@en ,
                      "TODO: Check whether this has to be maintained, as it does not seem to appear clearly in any of the conceptual or implementation models of Transmodel"@en ;
         rdfs:label "CheckIn"@en .


###  https://w3id.org/transmodel/facilities#CommercialService
:CommercialService rdf:type owl:Class ;
                   rdfs:subClassOf :LocalService ;
                   rdfs:comment "CommercialService is the specialisation of services for commercial purposes"@en ,
                                "TODO: Check if this has to be maintained as a classification or only keep them in a flat list, as it is proposed in the Equipment Overview Physical Model of Transmodel (figure 247)"@en ;
                   rdfs:label "CommercialService"@en .


###  https://w3id.org/transmodel/facilities#CommunicationService
:CommunicationService rdf:type owl:Class ;
                      rdfs:subClassOf :CommercialService ;
                      rdfs:comment "Specialisation of LocalService dedicated to communication services"@en ;
                      rdfs:label "CommunicationService"@en .


###  https://w3id.org/transmodel/facilities#ComplaintsService
:ComplaintsService rdf:type owl:Class ;
                   rdfs:subClassOf :CustomerService ;
                   rdfs:comment "Specialisation of CustomerService for Complaints Services"@en ;
                   rdfs:label "ComplaintsService"@en .


###  https://w3id.org/transmodel/facilities#Constraint
:Constraint rdf:type owl:Class ;
            rdfs:subClassOf :THINGSTOREVIEW ;
            rdfs:comment "A constraint that can take place at a SiteComponent that may potentially incur a time penalty that should be allowed for when journey planning"@en ,
                         "Constraint"@en .


###  https://w3id.org/transmodel/facilities#ConstraintDelay
:ConstraintDelay rdf:type owl:Class ;
                 rdfs:subClassOf :Constraint ;
                 rdfs:comment "A time penalty associated with a Constraint"@en ;
                 rdfs:label "ConstraintDelay"@en .


###  https://w3id.org/transmodel/facilities#ConstraintOfAccess
:ConstraintOfAccess rdf:type owl:Class ;
                    rdfs:subClassOf :Constraint ;
                    rdfs:comment "Access feature for CheckConstraint"@en ;
                    rdfs:label "ConstraintOfAccess"@en .


###  https://w3id.org/transmodel/facilities#ConstraintThroughput
:ConstraintThroughput rdf:type owl:Class ;
                      rdfs:subClassOf :Constraint ;
                      rdfs:comment "ConstraintThroughput is the throughput of a Constraint: the number of passenger who can pass through it in a specified interval"@en ;
                      rdfs:label "ConstraintThroughput"@en .


###  https://w3id.org/transmodel/facilities#CrossingEquipment
:CrossingEquipment rdf:type owl:Class ;
                   rdfs:subClassOf :AccessEquipment ;
                   rdfs:comment """Specialisation of PlaceAccessEquipment for CrossingEquipment

- Zebra"""@en ;
                   rdfs:label "CrossingEquipment"@en .


###  https://w3id.org/transmodel/facilities#CrossingEquipmentLights
:CrossingEquipmentLights rdf:type owl:Class ;
                         rdfs:subClassOf :CrossingEquipment ;
                         rdfs:comment "TODO: Check if this has to be maintained, as it is not present in the Equipment Overview Physical Model of Transmodel (figure 247)"@en .


###  https://w3id.org/transmodel/facilities#CrossingEquipmentPedestrian
:CrossingEquipmentPedestrian rdf:type owl:Class ;
                             rdfs:subClassOf :CrossingEquipment ;
                             rdfs:comment "TODO: Check if this has to be maintained, as it is not present in the Equipment Overview Physical Model of Transmodel (figure 247)"@en .


###  https://w3id.org/transmodel/facilities#CrossingEquipmentTactileGuideStrip
:CrossingEquipmentTactileGuideStrip rdf:type owl:Class ;
                                    rdfs:subClassOf :CrossingEquipment ;
                                    rdfs:comment "TODO: Check if this has to be maintained, as it is not present in the Equipment Overview Physical Model of Transmodel (figure 247)"@en .


###  https://w3id.org/transmodel/facilities#CrossingEquipmentZebra
:CrossingEquipmentZebra rdf:type owl:Class ;
                        rdfs:subClassOf :CrossingEquipment ;
                        rdfs:comment "TODO: Check if this has to be maintained, as it is not present in the Equipment Overview Physical Model of Transmodel (figure 247)"@en .


###  https://w3id.org/transmodel/facilities#CustomerService
:CustomerService rdf:type owl:Class ;
                 rdfs:subClassOf :LocalService ;
                 rdfs:comment "Generic specialisation of LocalService for CustomerServices (LostProperties, MeetingPoint, Complaiants, etc.)"@en ;
                 rdfs:label "CustomerService"@en .


###  https://w3id.org/transmodel/facilities#CycleOperatingEquipment
:CycleOperatingEquipment rdf:type owl:Class ;
                         rdfs:subClassOf :PlaceEquipment ;
                         rdfs:comment "A specialisation of PlaceEquipment describing cycle parking equipment"@en ,
                                      "TODO: Check if this has to be maintained, as it is not present in the Equipment Overview Physical Model of Transmodel (figure 247)"@en ;
                         rdfs:label "CycleStorageEquipment"@en .


###  https://w3id.org/transmodel/facilities#EmergencyService
:EmergencyService rdf:type owl:Class ;
                  rdfs:subClassOf :LocalService ;
                  rdfs:comment "TODO: Check if this has to be maintained, as it is not present in the Equipment Overview Physical Model of Transmodel (figure 247)"@en ;
                  rdfs:label "EmergencyService"@en .


###  https://w3id.org/transmodel/facilities#EncumbranceNeed
:EncumbranceNeed rdf:type owl:Class ;
                 rdfs:subClassOf :UserNeed ;
                 rdfs:comment "A specific UserNeed, i.e. a requirement of a Passenger travelling with luggage, animal or any other object requiring special arrangements to access PublicTransport"@en ;
                 rdfs:label "EncumbranceNeed"@en .


###  https://w3id.org/transmodel/facilities#Entrance
:Entrance rdf:type owl:Class ;
          rdfs:comment "A physical entrance or exit to/from a Site. May be a door, barrier, gate or other recognizable Point of Access."@en ;
          rdfs:label "Entrance"@en .


###  https://w3id.org/transmodel/facilities#EntranceEquipment
:EntranceEquipment rdf:type owl:Class ;
                   rdfs:subClassOf :AccessEquipment ;
                   rdfs:comment "Specialisation of PlaceAccessEquipment for Entrances (door, barrier, gate or other recognizable point of access)"@en ;
                   rdfs:label "EntranceEquipment"@en .


###  https://w3id.org/transmodel/facilities#Equipment
:Equipment rdf:type owl:Class ;
           rdfs:subClassOf [ rdf:type owl:Restriction ;
                             owl:onProperty :equipmentType ;
                             owl:allValuesFrom [ owl:intersectionOf ( <http://www.w3.org/2004/02/skos/core#Concept>
                                                                      [ rdf:type owl:Restriction ;
                                                                        owl:onProperty <http://www.w3.org/2004/02/skos/core#inScheme> ;
                                                                        owl:hasValue <https://w3id.org/transmodel/kos/facilities/EquipmentType>
                                                                      ]
                                                                    ) ;
                                                 rdf:type owl:Class
                                               ]
                           ] ,
                           [ rdf:type owl:Restriction ;
                             owl:onProperty :locatedIn ;
                             owl:maxQualifiedCardinality "1"^^xsd:nonNegativeInteger ;
                             owl:onClass :EquipmentPlace
                           ] ,
                           [ rdf:type owl:Restriction ;
                             owl:onProperty :outOfService ;
                             owl:maxQualifiedCardinality "1"^^xsd:nonNegativeInteger ;
                             owl:onDataRange xsd:boolean
                           ] ;
           rdfs:comment """An equipment that may be located on a Vehicle, Site, etc. There are many different types of equipment, each of which may have specific properties (hence a large classification of concepts is provided as subclasses of this class).

The two main specialisations are Local Service and Installed Equipment.

A Local Service is an intangible service that is provided at a site, such as selling tickets, porterage, etc.

An Installed Equipment is the fixed equipment that may be installed fixed on a site (Place Equipment - e.g., door, lift, gate, etc.) or a vehicle (Vehicle Equipment), or mixed (e.g., rubish bins, sanitary equipment or ticketing equipments).

These are further characterised as Place Equipment (equipment which may be located only on a SITE, such as a barrier, bench, lift) and Passenger Equipment (equipment which may be located on either a Vehicle or a Site, such as a display terminal, ticket validator or WC)"""@en ;
           rdfs:label "Equipment"@en .


###  https://w3id.org/transmodel/facilities#EquipmentPlace
:EquipmentPlace rdf:type owl:Class ;
                rdfs:subClassOf :SiteComponent ,
                                [ rdf:type owl:Restriction ;
                                  owl:onProperty :equippedWith ;
                                  owl:allValuesFrom :Equipment
                                ] ,
                                [ rdf:type owl:Restriction ;
                                  owl:onProperty :position ;
                                  owl:allValuesFrom :EquipmentPosition
                                ] ;
                rdfs:comment "An Equipment Place is a Site Component containing Equipment" ;
                rdfs:label "Equipment Place" .


###  https://w3id.org/transmodel/facilities#EquipmentPosition
:EquipmentPosition rdf:type owl:Class ;
                   rdfs:comment "TODO: Add a geolocation property for the position (most probably it will be a GeoSPARQL property, or a relationship to geo:Point)"@en ,
                                "The position that an equipment has, which comes with geospatial information and a description"@en ;
                   rdfs:label "Equipment Position"@en .


###  https://w3id.org/transmodel/facilities#EscalatorEquipment
:EscalatorEquipment rdf:type owl:Class ;
                    rdfs:subClassOf :StairEquipment ;
                    rdfs:comment "Specialisation of StairEquipment for Escalator Equipment"@en ;
                    rdfs:label "EscalatorEquipment"@en .


###  https://w3id.org/transmodel/facilities#Facility
:Facility rdf:type owl:Class ;
          rdfs:subClassOf [ rdf:type owl:Restriction ;
                            owl:onProperty :facilityType ;
                            owl:allValuesFrom [ owl:intersectionOf ( <http://www.w3.org/2004/02/skos/core#Concept>
                                                                     [ rdf:type owl:Restriction ;
                                                                       owl:onProperty <http://www.w3.org/2004/02/skos/core#inScheme> ;
                                                                       owl:hasValue <https://w3id.org/transmodel/kos/facilities/FacilityType>
                                                                     ]
                                                                   ) ;
                                                rdf:type owl:Class
                                              ]
                          ] ;
          rdfs:comment """A named amenity available to the public at a Site or on a Service.

A Facility has a type that determines the type of facility that it refers to, available in the SKOS codelist https://w3id.org/transmodel/kos/facilities/facilityType (in Netex this is represented as a set of enumerations)

A Facility has no further properties than a name. An Equipment or LocalService is used to describe the further properties provided as part of a particular Facility"""@en ;
          rdfs:label "Facility"@en .


###  https://w3id.org/transmodel/facilities#FacilitySet
:FacilitySet rdf:type owl:Class ;
             rdfs:subClassOf [ rdf:type owl:Restriction ;
                               owl:onProperty :comprisesEquipment ;
                               owl:allValuesFrom :Equipment
                             ] ,
                             [ rdf:type owl:Restriction ;
                               owl:onProperty :comprisesFacility ;
                               owl:allValuesFrom :Facility
                             ] ;
             rdfs:comment """A facility set is an aggregation of facilities. In Netex this is represented as a set of enumerated facility values (names based on TPEG classifications, augmented with UIC etc.).
The terms used for relating a facility set to the facilities and equipment are CommonFacilityGroup and otherFacilities. We have preferred using comprisesFacility and comprisesEquipment to simplify the terminology that is being used."""@en ,
                          "TODO: Add a restriction in subclassof for :providedBy only org:Organization"@en ,
                          "TODO: Transmodel also identifies as a potential restriction the assignment of 0 to N validity conditions to the Facility Set, but this has not been yet modelled"@en ;
             rdfs:label "Facility Set"@en .


###  https://w3id.org/transmodel/facilities#FlexibleStopPlace
:FlexibleStopPlace rdf:type owl:Class ;
                   rdfs:subClassOf :StopPlace ;
                   rdfs:comment "A specialisation of the Stop Place describing a stop of a Flexible Service. It may be composed of Flexible Areas or Hail and Ride Areas identifying the catchment areas for flexible services (when they use areas or flexible quays). Some Flexible Places also use regular Stop Places for their stops. When assigned to a Scheduled Stop Point the corresponding Scheduled Stop Point is supposed to be a Zone (the centroid point of the Zone being the Scheduled Stop Point)."@en ;
                   rdfs:label "Flexible Stop Place"@en .


###  https://w3id.org/transmodel/facilities#FreeWifi
:FreeWifi rdf:type owl:Class ;
          rdfs:subClassOf :CommunicationService ;
          rdfs:comment "A private WiFi network that is available under certain characteristics"@en ,
                       "TODO: Check if this has to be maintained, as it is not present in the Equipment Overview Physical Model of Transmodel (figure 247)"@en ;
          rdfs:label "FreeWifi"@en .


###  https://w3id.org/transmodel/facilities#Garage
:Garage rdf:type owl:Class ;
        rdfs:subClassOf :PlaceEquipment ;
        rdfs:comment """A Facility of PlaceEquipment used for parking and maintaining
	vehicles. Parking Point in a Garage are called GaragePoint."""@en ,
                     "TODO: Check if this has to be maintained, as it is not present in the Equipment Overview Physical Model of Transmodel (figure 247)"@en ;
        rdfs:label "Garage"@en .


###  https://w3id.org/transmodel/facilities#HeadingSign
:HeadingSign rdf:type owl:Class ;
             rdfs:subClassOf :SignEquipment ;
             rdfs:comment "Specialisation of SignEquipment for headings providing information like direction name, line name, etc."@en ;
             rdfs:label "HeadingSign"@en .


###  https://w3id.org/transmodel/facilities#HiringService
:HiringService rdf:type owl:Class ;
               rdfs:subClassOf :CommercialService ;
               rdfs:comment "HiringService is the specialisation of CommercialService for hiring services"@en ;
               rdfs:label "HiringService"@en .


###  https://w3id.org/transmodel/facilities#Immigration
:Immigration rdf:type owl:Class ;
             rdfs:subClassOf :EquipmentPlace ;
             rdfs:comment "One specialisation of SiteComponent for Migration affaires"@en ,
                          "TODO: Check whether this has to be maintained, as it does not seem to appear clearly in any of the conceptual or implementation models of Transmodel"@en ;
             rdfs:label "Immigration"@en .


###  https://w3id.org/transmodel/facilities#InformationBooklet
:InformationBooklet rdf:type owl:Class ;
                    rdfs:subClassOf :PassengerInformationPrintedMaterial ;
                    rdfs:comment "Information Booklet is public transport piece of Equipment dedicated to inform"@en ,
                                 "TODO: Check if this has to be maintained, as it is not present in the Equipment Overview Physical Model of Transmodel (figure 247)"@en ;
                    rdfs:label "InformationBooklet"@en .


###  https://w3id.org/transmodel/facilities#InformationLeaflet
:InformationLeaflet rdf:type owl:Class ;
                    rdfs:subClassOf :PassengerInformationPrintedMaterial ;
                    rdfs:comment "A public transport information piece of Equipment"@en ,
                                 "TODO: Check if this has to be maintained, as it is not present in the Equipment Overview Physical Model of Transmodel (figure 247)"@en ;
                    rdfs:label "InformationLeaflet"@en .


###  https://w3id.org/transmodel/facilities#InstalledEquipment
:InstalledEquipment rdf:type owl:Class ;
                    rdfs:subClassOf :Equipment ;
                    rdfs:comment """An Installed Equipment is a fixed equipment that may be installed on a site (such as a door, lift, gate, etc.) or a vehicle. Its exact location may be specified by an Equipment Place. 
Physical equipments installed either fixed (PlaceEquipment), on-board (VehicleEquipment) or mixed (some equipments as rubish, sanitary or ticketing)."""@en ;
                    rdfs:label "Installed Equipment"@en .


###  https://w3id.org/transmodel/facilities#JourneyPattern
:JourneyPattern rdf:type owl:Class ;
                rdfs:subClassOf :THINGSTOREVIEW ;
                rdfs:label "JourneyPattern"@en .


###  https://w3id.org/transmodel/facilities#LeftLuggageService
:LeftLuggageService rdf:type owl:Class ;
                    rdfs:subClassOf :LuggageService ;
                    rdfs:comment "LeftLuggageService is the implementation of LuggageService for LeftLuggageService"@en ;
                    rdfs:label "LeftLuggageService"@en .


###  https://w3id.org/transmodel/facilities#LiftEquipment
:LiftEquipment rdf:type owl:Class ;
               rdfs:subClassOf :AccessEquipment ;
               rdfs:comment "Specialisation of PlaceAccessEquipment dedicated to PlaceAccessLift"@en ;
               rdfs:label "PlaceAccessLift"@en .


###  https://w3id.org/transmodel/facilities#LocalService
:LocalService rdf:type owl:Class ;
              rdfs:subClassOf :Equipment ;
              rdfs:comment """A Service (LocalService such as LeftLuggage, TicketingService) is considered as immaterial Equipment as well.

A named Service relating to the use of the Site or transport Services at a particular location, for example Porterage, AssistanceForDissabledUsers, BookingOffices, etc. The Service may have a validityCondition associated with it."""@en ;
              rdfs:label "Service"@en .


###  https://w3id.org/transmodel/facilities#LostPropertieService
:LostPropertieService rdf:type owl:Class ;
                      rdfs:subClassOf :CustomerService ;
                      rdfs:comment "Specialisation of CustomerService for LostProperties"@en ;
                      rdfs:label "LostProperties"@en .


###  https://w3id.org/transmodel/facilities#LowFloor
:LowFloor rdf:type owl:Class ;
          rdfs:subClassOf :VehicleAccessEquipment ;
          rdfs:comment "Specialisation of VehicleAccessEquipment dedicated to LowFloor"@en ,
                       "TODO: Check if this has to be maintained, as it is not present in the Equipment Overview Physical Model of Transmodel (figure 247)"@en ;
          rdfs:label "LowFloor"@en .


###  https://w3id.org/transmodel/facilities#LuggageLockerEquipment
:LuggageLockerEquipment rdf:type owl:Class ;
                        rdfs:subClassOf :SiteEquipment ;
                        rdfs:comment "Specialisation of LuggageLockerEquipment for StopPlaceEquipment"@en ;
                        rdfs:label "LuggageLockerEquipment"@en .


###  https://w3id.org/transmodel/facilities#LuggageService
:LuggageService rdf:type owl:Class ;
                rdfs:subClassOf :CustomerService ;
                rdfs:comment """Specialisation of CustomerServices for LuggageServices.

Provides facilities as LuggageTrolley, FreeToUse, etc."""@en ,
                             "TODO: Check if this has to be maintained or moved to LocalService, as it is  present elsehwere in the Equipment Overview Physical Model of Transmodel (figure 247)"@en ;
                rdfs:label "LuggageService"@en .


###  https://w3id.org/transmodel/facilities#LuggageTrolleyService
:LuggageTrolleyService rdf:type owl:Class ;
                       rdfs:subClassOf :LuggageService ;
                       rdfs:comment "TODO: Check if this has to be maintained, as it is not present in the Equipment Overview Physical Model of Transmodel (figure 247)"@en ;
                       rdfs:label "LuggageTrolley"@en ,
                                  "Specialisation of LuggageServices for LuggageTrolleyServices"@en .


###  https://w3id.org/transmodel/facilities#MeetingPointService
:MeetingPointService rdf:type owl:Class ;
                     rdfs:subClassOf :CustomerService ;
                     rdfs:comment "Specialisation of CustomerService for meeting points (provides characteristics like description, labels...)"@en ;
                     rdfs:label "MeetingPointService"@en .


###  https://w3id.org/transmodel/facilities#MoneyService
:MoneyService rdf:type owl:Class ;
              rdfs:subClassOf :CommercialService ;
              rdfs:comment "MoneyService is the specialisation of Commercial services for money services. Provides information about money services."@en ;
              rdfs:label "MoneyService"@en .


###  https://w3id.org/transmodel/facilities#Notice
:Notice rdf:type owl:Class ;
        rdfs:subClassOf :THINGSTOREVIEW ;
        rdfs:comment "A text for informational purposes on exceptions in a Line, a Journey Pattern, etc. The information may be usable for Passenger or driver information"@en ;
        rdfs:label "Notice"@en .


###  https://w3id.org/transmodel/facilities#OnboardStay
:OnboardStay rdf:type owl:Class ;
             rdfs:subClassOf :Facility ,
                             [ rdf:type owl:Restriction ;
                               owl:onProperty :boardingPermission ;
                               owl:maxQualifiedCardinality "1"^^xsd:nonNegativeInteger ;
                               owl:onClass [ owl:intersectionOf ( <http://www.w3.org/2004/02/skos/core#Concept>
                                                                  [ rdf:type owl:Restriction ;
                                                                    owl:onProperty <http://www.w3.org/2004/02/skos/core#inScheme> ;
                                                                    owl:hasValue <https://w3id.org/transmodel/kos/facilities/FacilityType>
                                                                  ]
                                                                ) ;
                                             rdf:type owl:Class
                                           ]
                             ] ,
                             [ rdf:type owl:Restriction ;
                               owl:onProperty :fareClass ;
                               owl:maxQualifiedCardinality "1"^^xsd:nonNegativeInteger ;
                               owl:onClass [ owl:intersectionOf ( <http://www.w3.org/2004/02/skos/core#Concept>
                                                                  [ rdf:type owl:Restriction ;
                                                                    owl:onProperty <http://www.w3.org/2004/02/skos/core#inScheme> ;
                                                                    owl:hasValue <https://w3id.org/transmodel/kos/facilities/FacilityType>
                                                                  ]
                                                                ) ;
                                             rdf:type owl:Class
                                           ]
                             ] ,
                             [ rdf:type owl:Restriction ;
                               owl:onProperty :duration ;
                               owl:maxQualifiedCardinality "1"^^xsd:nonNegativeInteger ;
                               owl:onDataRange xsd:duration
                             ] ;
             rdfs:comment "This is a type of Service Facility Set, according to the Facility Conceptual Model (figure 287, page 450) of TransModel"@en ;
             rdfs:label "Onboard Stay"@en .


###  https://w3id.org/transmodel/facilities#OtherSign
:OtherSign rdf:type owl:Class ;
           rdfs:subClassOf :SignEquipment ;
           rdfs:comment "Specialisation of SignEquipment which are not HeadingSign nor PlaceSign"@en ;
           rdfs:label "Other Sign"@en .


###  https://w3id.org/transmodel/facilities#Passenger
:Passenger rdf:type owl:Class ;
           rdfs:subClassOf :THINGSTOREVIEW ;
           rdfs:comment "The Person who uses Public Transport Services"@en ;
           rdfs:label "Passenger"@en .


###  https://w3id.org/transmodel/facilities#PassengerArea
:PassengerArea rdf:type owl:Class ;
               rdfs:subClassOf :THINGSTOREVIEW ;
               rdfs:comment """A Passenger Area within a StopPlace such as:
- Concourse
- Booking Hall
- Immigration Hall
- Security Area

Accessible by Passenger but without direct access to Vehicles"""@en ;
               rdfs:label "PassengerArea"@en .


###  https://w3id.org/transmodel/facilities#PassengerEquipment
:PassengerEquipment rdf:type owl:Class ;
                    rdfs:subClassOf :InstalledEquipment ,
                                    [ rdf:type owl:Restriction ;
                                      owl:onProperty :locatedIn ;
                                      owl:maxQualifiedCardinality "1"^^xsd:nonNegativeInteger ;
                                      owl:onClass [ rdf:type owl:Class ;
                                                    owl:unionOf ( :EquipmentPlace
                                                                  :Vehicle
                                                                )
                                                  ]
                                    ] ,
                                    [ rdf:type owl:Restriction ;
                                      owl:onProperty :fixed ;
                                      owl:maxQualifiedCardinality "1"^^xsd:nonNegativeInteger ;
                                      owl:onDataRange xsd:boolean
                                    ] ;
                    rdfs:comment "An item of equipment of a particular type actually available at a location within a Place (fixed) or a Vehicle (onboard)"@en ;
                    rdfs:label "PassengerEquipment"@en .


###  https://w3id.org/transmodel/facilities#PassengerInformationEquipment
:PassengerInformationEquipment rdf:type owl:Class ;
                               rdfs:subClassOf :PassengerEquipment ;
                               rdfs:comment "A public transport information piece of Equipment, as for instance terminals (on street, at information desks, telematic,...) or printed material (leaflets displayed at Stops, booklets, ...)"@en ;
                               rdfs:label "PassengerInformationEquipment"@en .


###  https://w3id.org/transmodel/facilities#PassengerInformationPrintedMaterial
:PassengerInformationPrintedMaterial rdf:type owl:Class ;
                                     rdfs:subClassOf :PassengerInformationEquipment ;
                                     rdfs:comment "A public transport information piece of Equipment which is printed material (leaflets displayed at Stops, booklets, ...)"@en ,
                                                  "TODO: Check if this has to be maintained, as it is not present in the Equipment Overview Physical Model of Transmodel (figure 247)"@en ;
                                     rdfs:label "PassengerInformationPrintedMaterial"@en .


###  https://w3id.org/transmodel/facilities#PassengerInformationTerminal
:PassengerInformationTerminal rdf:type owl:Class ;
                              rdfs:subClassOf :PassengerInformationEquipment ;
                              rdfs:comment "A public transport information piece of equipment such as street stands, information desks or telematic services"@en ,
                                           "TODO: Check if this has to be maintained, as it is not present in the Equipment Overview Physical Model of Transmodel (figure 247)"@en ;
                              rdfs:label "PassengerInformationDesk"@en .


###  https://w3id.org/transmodel/facilities#PassengerSafetyEquipment
:PassengerSafetyEquipment rdf:type owl:Class ;
                          rdfs:subClassOf :PassengerEquipment ;
                          rdfs:label "PassengerSafetyEquipment"@en .


###  https://w3id.org/transmodel/facilities#PlaceEquipment
:PlaceEquipment rdf:type owl:Class ;
                rdfs:subClassOf :InstalledEquipment ,
                                [ owl:intersectionOf ( [ rdf:type owl:Restriction ;
                                                         owl:onProperty :position ;
                                                         owl:someValuesFrom :EquipmentPosition
                                                       ]
                                                       [ rdf:type owl:Restriction ;
                                                         owl:onProperty :position ;
                                                         owl:maxQualifiedCardinality "1"^^xsd:nonNegativeInteger ;
                                                         owl:onClass :EquipmentPosition
                                                       ]
                                                     ) ;
                                  rdf:type owl:Class
                                ] ,
                                [ rdf:type owl:Restriction ;
                                  owl:onProperty :fixed ;
                                  owl:hasValue "true"^^xsd:boolean
                                ] ;
                rdfs:comment "An item of Equipment of a particular type actually available at a location within a Place. It can only have one position"@en ;
                rdfs:label "PlaceEquipment"@en .


###  https://w3id.org/transmodel/facilities#PlaceLighting
:PlaceLighting rdf:type owl:Class ;
               rdfs:subClassOf :PlaceEquipment ;
               rdfs:comment "Place Lighting"@en .


###  https://w3id.org/transmodel/facilities#PlaceSign
:PlaceSign rdf:type owl:Class ;
           rdfs:subClassOf :SignEquipment ;
           rdfs:comment "SignEquipment withe the name of a Place on it"@en ;
           rdfs:label "PlaceSign"@en .


###  https://w3id.org/transmodel/facilities#Porterage
:Porterage rdf:type owl:Class ;
           rdfs:subClassOf :LocalService ;
           rdfs:comment "Porterage"@en ,
                        "PorterageService"@en ,
                        "TODO: Check if this has to be maintained, as it is not present in the Equipment Overview Physical Model of Transmodel (figure 247)"@en .


###  https://w3id.org/transmodel/facilities#PostOfficeService
:PostOfficeService rdf:type owl:Class ;
                   rdfs:subClassOf :CommunicationService ;
                   rdfs:comment "A PostOfficeService is the specialisation of CommunicationService for post mail services"@en ,
                                "TODO: Check if this has to be maintained, as it is not present in the Equipment Overview Physical Model of Transmodel (figure 247)"@en ;
                   rdfs:label "PostOfficeService"@en .


###  https://w3id.org/transmodel/facilities#Quay
:Quay rdf:type owl:Class ;
      rdfs:subClassOf [ rdf:type owl:Restriction ;
                        owl:onProperty <https://w3id.org/transmodel/commons#in> ;
                        owl:allValuesFrom :StopPlace
                      ] ,
                      [ rdf:type owl:Restriction ;
                        owl:onProperty :comprises ;
                        owl:allValuesFrom :Quay
                      ] ;
      rdfs:comment """A place such as platform, stance, or quayside where passengers have access to public transport vehicles, taxi, cars or other means of transportation. A Quay may serve one or more Vehicle Stopping Places and be associated with one or more Scheduled Stop Points. 

A Quay may contain other sub Quays"""@en ;
      rdfs:label "Quay"@en .


###  https://w3id.org/transmodel/facilities#QueuingEquipment
:QueuingEquipment rdf:type owl:Class ;
                  rdfs:subClassOf :AccessEquipment ;
                  rdfs:label "QueingEquipment"@en .


###  https://w3id.org/transmodel/facilities#Ramp
:Ramp rdf:type owl:Class ;
      rdfs:subClassOf :VehicleAccessEquipment ;
      rdfs:comment "Specialisation of VehicleAccessEquipment dedicated to VehicleRamp"@en ,
                   "TODO: Check if this has to be maintained, as it is not present in the Equipment Overview Physical Model of Transmodel (figure 247)"@en ;
      rdfs:label "VehicleRamp"@en .


###  https://w3id.org/transmodel/facilities#RampEquipment
:RampEquipment rdf:type owl:Class ;
               rdfs:subClassOf :AccessEquipment ;
               rdfs:comment "Specialisation of PlaceEquipment dedicated to access"@en ;
               rdfs:label "PlaceAccessRamp"@en .


###  https://w3id.org/transmodel/facilities#RetailService
:RetailService rdf:type owl:Class ;
               rdfs:subClassOf :CommercialService ;
               rdfs:comment "Specialisation of LocalService dedicated to retail services"@en ;
               rdfs:label "RetailService"@en .


###  https://w3id.org/transmodel/facilities#RoughSurface
:RoughSurface rdf:type owl:Class ;
              rdfs:subClassOf :PlaceEquipment ;
              rdfs:label "Rough Surface"@en .


###  https://w3id.org/transmodel/facilities#RubishDisposalEquipment
:RubishDisposalEquipment rdf:type owl:Class ;
                         rdfs:subClassOf :PassengerEquipment ;
                         rdfs:comment "Specialisation of Passenger Equipment for Rubish Disposal"@en ;
                         rdfs:label "RubishDisposal"@en .


###  https://w3id.org/transmodel/facilities#SanitaryEquipment
:SanitaryEquipment rdf:type owl:Class ;
                   rdfs:subClassOf :PassengerEquipment ;
                   rdfs:comment "Specialisation of Passenger Equipment for Sanitary Equipment"@en ;
                   rdfs:label "TypeOfSanitaryEquipment"@en .


###  https://w3id.org/transmodel/facilities#Screening
:Screening rdf:type owl:Class ;
           rdfs:subClassOf :EquipmentPlace ;
           rdfs:comment "One specialisation of SiteComponent for Security Screening"@en ,
                        "TODO: Check whether this has to be maintained, as it does not seem to appear clearly in any of the conceptual or implementation models of Transmodel"@en ;
           rdfs:label "SecurityScreening"@en .


###  https://w3id.org/transmodel/facilities#SeatingEquipment
:SeatingEquipment rdf:type owl:Class ;
                  rdfs:subClassOf :WaitingEquipment ;
                  rdfs:label "SeatingEquipment"@en .


###  https://w3id.org/transmodel/facilities#ServiceFacilitySet
:ServiceFacilitySet rdf:type owl:Class ;
                    rdfs:subClassOf :FacilitySet ,
                                    [ rdf:type owl:Restriction ;
                                      owl:onProperty :presentAt ;
                                      owl:allValuesFrom :VehicleType
                                    ] ;
                    rdfs:comment """A service facility set contains a set of facilities available for a service journey or a journey part. The set may be availabe only for a specific vehicle type within the service (e.g., carriage equipped with low floor).
It can also include information about the accommodation on board, which can be related to the Accommodation or OnboardStay concepts, which are subclasses of Facility, via the comprisesFacility object property. These two concepts are further refined since they may have additional attributes beyond the indication of the corresponding SKOS concepts, as in the other cases."""@en ,
                                 """TODO: Other class restrictions that may be added may include:
- for (inverse of made using), for Vehicle Journey and Coupled Journey (see figure 287, Facility conceptual Model)"""@en ;
                    rdfs:label "Service Facility Set"@en .

[ rdf:type owl:Axiom ;
   owl:annotatedSource :ServiceFacilitySet ;
   owl:annotatedProperty rdfs:subClassOf ;
   owl:annotatedTarget [ rdf:type owl:Restriction ;
                         owl:onProperty :presentAt ;
                         owl:allValuesFrom :VehicleType
                       ] ;
   rdfs:comment "See figure 287, Facility conceptual Model"
 ] .


###  https://w3id.org/transmodel/facilities#ShelterEquipment
:ShelterEquipment rdf:type owl:Class ;
                  rdfs:subClassOf :WaitingEquipment ;
                  rdfs:comment "A building or other structure constructed at a Bus Stop"@en ;
                  rdfs:label "Shelter"@en .


###  https://w3id.org/transmodel/facilities#Shower
:Shower rdf:type owl:Class ;
        rdfs:subClassOf :SanitaryEquipment ;
        rdfs:comment "Specialisation of SanitaryEquipment for showers"@en ,
                     "TODO: Check if this has to be maintained, as it is not present in the Equipment Overview Physical Model of Transmodel (figure 247)"@en ;
        rdfs:label "Shower"@en .


###  https://w3id.org/transmodel/facilities#SignEquipment
:SignEquipment rdf:type owl:Class ;
               rdfs:subClassOf :PlaceEquipment ;
               rdfs:comment "Specialisation of PlaceEquipment for Signs"@en ;
               rdfs:label "SignEquipment"@en .


###  https://w3id.org/transmodel/facilities#Site
:Site rdf:type owl:Class ;
      rdfs:subClassOf [ rdf:type owl:Restriction ;
                        owl:onProperty :concernedBy ;
                        owl:allValuesFrom :FacilitySet
                      ] ;
      rdfs:comment "A well known Place to which Passengers may refer to indicate the origin or a destination of a Trip"@en ;
      rdfs:label "Site"@en .


###  https://w3id.org/transmodel/facilities#SiteComponent
:SiteComponent rdf:type owl:Class ;
               rdfs:subClassOf :SiteElement ;
               rdfs:comment "An element of a Site describing a part of its structure. Site Components share common properties for data management, accessibility and other features"@en ;
               rdfs:label "Site Component"@en .


###  https://w3id.org/transmodel/facilities#SiteElement
:SiteElement rdf:type owl:Class ;
             rdfs:subClassOf [ rdf:type owl:Restriction ;
                               owl:onProperty :accessibilityAssessment ;
                               owl:maxQualifiedCardinality "1"^^xsd:nonNegativeInteger ;
                               owl:onClass :AccessibilityAssessment
                             ] ;
             rdfs:comment "A place"@en ,
                          "TODO: Although the Transmodel conceptual model on Site Equipment specifies that a Site Element can only have one accessibility assessment, this may need to be relaxed to allow for more values to be included."@en ,
                          "TODO: Check whether this should be related to a more general concept defining a place"@en ;
             rdfs:label "Site Element"@en .


###  https://w3id.org/transmodel/facilities#SiteEquipment
:SiteEquipment rdf:type owl:Class ;
               rdfs:subClassOf :PlaceEquipment ;
               rdfs:comment "Specialisation of PlaceEquipment for Site" ;
               rdfs:label "SiteEquipment" .


###  https://w3id.org/transmodel/facilities#SiteFacilitySet
:SiteFacilitySet rdf:type owl:Class ;
                 rdfs:subClassOf :FacilitySet ,
                                 [ rdf:type owl:Restriction ;
                                   owl:onProperty :availableAt ;
                                   owl:allValuesFrom :Site
                                 ] ;
                 rdfs:comment "A site facility set contains a set of facilities available at a site"@en ;
                 rdfs:label "Site Facility Set"@en .


###  https://w3id.org/transmodel/facilities#StairCaseEquipment
:StairCaseEquipment rdf:type owl:Class ;
                    rdfs:subClassOf :StairEquipment ;
                    rdfs:comment "Specialisation of PlaceAccessStair for StairCaseEquipment"@en ;
                    rdfs:label "StairCaseEquipment"@en .


###  https://w3id.org/transmodel/facilities#StairEquipment
:StairEquipment rdf:type owl:Class ;
                rdfs:subClassOf :AccessEquipment ;
                rdfs:comment "Specialisation of PlaceAccessEquipment dedicated to PlaceAccessStair (stair, escalator, staircase, etc.)"@en ;
                rdfs:label "PlaceAccessStair"@en .


###  https://w3id.org/transmodel/facilities#StatusOfEquipment
:StatusOfEquipment rdf:type owl:Class ;
                   rdfs:subClassOf :THINGSTOREVIEW ;
                   rdfs:label "StatusOfEquipment"@en .


###  https://w3id.org/transmodel/facilities#StopPlace
:StopPlace rdf:type owl:Class ;
           rdfs:subClassOf :Site ,
                           [ rdf:type owl:Restriction ;
                             owl:onProperty :accessedBy ;
                             owl:allValuesFrom :StopPlaceEntrance
                           ] ,
                           [ rdf:type owl:Restriction ;
                             owl:onProperty :containing ;
                             owl:allValuesFrom :Quay
                           ] ,
                           [ rdf:type owl:Restriction ;
                             owl:onProperty <https://w3id.org/transmodel/commons#borderCrossing> ;
                             owl:allValuesFrom xsd:boolean
                           ] ;
           rdfs:comment "A place comprising one or more locations where Vehicles may stop and where passengers may board or leave Vehicles or prepare their Trip. A Stop Place will usually have one or more well-known names."@en ,
                        "TODO: Add Stop Place Components to the Stop Place, if considered useful."@en ,
                        "TODO: Add Stop Place Type as a SKOS Concept Scheme, and connect it to such concept scheme via an object property"@en ,
                        "TODO: If considered relevant, add connections from this class to the classes Point of Interest (this stop place services such Point of Interest) and to the class StopPlaceVehicleEntrance (this stop place is entered through an entrance - typical in an interchange area)."@en ;
           rdfs:label "Stop Place"@en .


###  https://w3id.org/transmodel/facilities#StopPlaceComponent
:StopPlaceComponent rdf:type owl:Class ;
                    rdfs:subClassOf :THINGSTOREVIEW ;
                    rdfs:comment "An element of a StopPlace describing part of its structure. StopPlaceComponent share common properties for data management, accessibility and other features"@en ;
                    rdfs:label "StopPlaceComponent"@en .


###  https://w3id.org/transmodel/facilities#StopPlaceEntrance
:StopPlaceEntrance rdf:type owl:Class ;
                   rdfs:subClassOf :Entrance ;
                   rdfs:comment "A physical Entrance or Exit to/from a Stop Place for a Passenger. May be a door, barrier, gate or other recognizable point of access."@en ;
                   rdfs:label "Stop Place Entrance"@en .


###  https://w3id.org/transmodel/facilities#StopPlaceSpace
:StopPlaceSpace rdf:type owl:Class ;
                rdfs:subClassOf :THINGSTOREVIEW ;
                rdfs:comment "A physical area within a StopPlace, for example, a Quay, BoardingPosition, AccessSpace or EquipmentPlace"@en ;
                rdfs:label "StopPlaceSpace"@en .


###  https://w3id.org/transmodel/facilities#Suitability
:Suitability rdf:type owl:Class ;
             rdfs:subClassOf :THINGSTOREVIEW ;
             rdfs:comment "A statement of whether a particular UserNeed can be met. It can be used to state whether a Site can accessed by a Passenger with a particular UserNeed."@en ;
             rdfs:label "Suitability"@en .


###  https://w3id.org/transmodel/facilities#THINGSTOREVIEW
:THINGSTOREVIEW rdf:type owl:Class .


###  https://w3id.org/transmodel/facilities#TicketControl
:TicketControl rdf:type owl:Class ;
               rdfs:subClassOf :EquipmentPlace ;
               rdfs:comment "One specialisation of SiteComponent for Ticket control"@en ,
                            "TODO: Check whether this has to be maintained, as it does not seem to appear clearly in any of the conceptual or implementation models of Transmodel"@en ;
               rdfs:label "TicketControl"@en .


###  https://w3id.org/transmodel/facilities#TicketValidatorEquipment
:TicketValidatorEquipment rdf:type owl:Class ;
                          rdfs:subClassOf :PassengerEquipment ;
                          rdfs:comment "Specialisation of Passenger Equipment for Ticket Validator Equipment"@en ;
                          rdfs:label "TicketValidatorEquipment"@en .


###  https://w3id.org/transmodel/facilities#TicketingEquipment
:TicketingEquipment rdf:type owl:Class ;
                    rdfs:subClassOf :PassengerEquipment ;
                    rdfs:comment "Specialisation of Passenter Equipment for Ticketing Equipment"@en ;
                    rdfs:label "TicketingEquipment"@en .


###  https://w3id.org/transmodel/facilities#TicketingService
:TicketingService rdf:type owl:Class ;
                  rdfs:subClassOf :LocalService ;
                  rdfs:label "TicketingService"@en .


###  https://w3id.org/transmodel/facilities#Toilet
:Toilet rdf:type owl:Class ;
        rdfs:subClassOf :SanitaryEquipment ;
        rdfs:comment "TODO: Check if this has to be maintained, as it is not present in the Equipment Overview Physical Model of Transmodel (figure 247)"@en ;
        rdfs:label "Toilet"@en .


###  https://w3id.org/transmodel/facilities#TravelatorEquipment
:TravelatorEquipment rdf:type owl:Class ;
                     rdfs:subClassOf :AccessEquipment .


###  https://w3id.org/transmodel/facilities#TrolleyStandEquipment
:TrolleyStandEquipment rdf:type owl:Class ;
                       rdfs:subClassOf :SiteEquipment ;
                       rdfs:comment "Specialisation of StopPlaceEquipment for trolley stands"@en ;
                       rdfs:label "TrolleyStandEquipment"@en .


###  https://w3id.org/transmodel/facilities#UserNeed
:UserNeed rdf:type owl:Class ;
          rdfs:subClassOf :THINGSTOREVIEW ;
          rdfs:comment "A users's need for a particular Suitability"@en ;
          rdfs:label "UserNeed"@en .


###  https://w3id.org/transmodel/facilities#ValidityCondition
:ValidityCondition rdf:type owl:Class ;
                   rdfs:subClassOf :THINGSTOREVIEW ;
                   rdfs:comment "Condition used in order to characterise a given Version of a VersionFrame. A ValidityCondition consists of a parameter (e.g. date, triggering event, etc.) and its type of application (e.g. for, from, until, etc.)"@en ;
                   rdfs:label "ValidityCondition"@en .


###  https://w3id.org/transmodel/facilities#ValidityRuleParameter
:ValidityRuleParameter rdf:type owl:Class ;
                       rdfs:subClassOf :ValidityCondition ;
                       rdfs:comment "A user defined ValidityCondition used by a rule for selecting versions. E.g. river level > 1.5 m. and bad weather"@en ;
                       rdfs:label "ValidityRuleParameter"@en .


###  https://w3id.org/transmodel/facilities#ValidityTrigger
:ValidityTrigger rdf:type owl:Class ;
                 rdfs:subClassOf :THINGSTOREVIEW ;
                 rdfs:comment "External event defining a ValidityCondition. T. g. exceptional flow of a river, bad weather, road closure for works"@en ;
                 rdfs:label "ValidityTrigger"@en .


###  https://w3id.org/transmodel/facilities#Vehicle
:Vehicle rdf:type owl:Class ;
         rdfs:subClassOf :THINGSTOREVIEW ;
         rdfs:comment "A PublicTransportVehicle used for carrying Passenger"@en ;
         rdfs:label "Vehicle"@en .


###  https://w3id.org/transmodel/facilities#VehicleAccessEquipment
:VehicleAccessEquipment rdf:type owl:Class ;
                        rdfs:subClassOf :VehicleEquipment ;
                        rdfs:comment "Specialisation of VehicleEquipment dedicated to access Vehicles providing information such as low floor, ramp, access area dimensions, etc."@en ;
                        rdfs:label "VehicleAccessEquipment"@en .


###  https://w3id.org/transmodel/facilities#VehicleChargingEquipment
:VehicleChargingEquipment rdf:type owl:Class ;
                          rdfs:subClassOf :PlaceEquipment ;
                          rdfs:comment "Specialisation of PlaceEquipment for Vehicle charging"@en ;
                          rdfs:label "VehicleChargingEquipment"@en .


###  https://w3id.org/transmodel/facilities#VehicleDisplayEquipment
:VehicleDisplayEquipment rdf:type owl:Class ;
                         rdfs:subClassOf :PassengerInformationEquipment ;
                         rdfs:comment "TODO: Check if this has to be maintained, as it is not present in the Equipment Overview Physical Model of Transmodel (figure 247)"@en ;
                         rdfs:label "PassengerInformationOnBoard"@en .


###  https://w3id.org/transmodel/facilities#VehicleEquipment
:VehicleEquipment rdf:type owl:Class ;
                  rdfs:subClassOf :InstalledEquipment ,
                                  [ rdf:type owl:Restriction ;
                                    owl:onProperty :locatedIn ;
                                    owl:maxQualifiedCardinality "1"^^xsd:nonNegativeInteger ;
                                    owl:onClass :Vehicle
                                  ] ;
                  rdfs:comment "A fixed equipment installed on a vehice. In Transmodel, this concept is called Actual Vehicle Equipment"@en ,
                               "TODO: check whether the range of the property locatedIn should go into the concept Vehicle from a different module of the ontology"@en ;
                  rdfs:label "Vehicle Equipment"@en .


###  https://w3id.org/transmodel/facilities#VehicleMode
:VehicleMode rdf:type owl:Class ;
             rdfs:subClassOf :Vehicle ;
             rdfs:comment "A classification of Public Transport Vehicles of the same Vehicle Type, e.g. according to Equipment specifications or model generation."@en ;
             rdfs:label "VehicleModel"@en .


###  https://w3id.org/transmodel/facilities#VehicleStoppingPlace
:VehicleStoppingPlace rdf:type owl:Class ;
                      rdfs:subClassOf :THINGSTOREVIEW ;
                      rdfs:comment """A place on the vehicle track where vehicles stop in order for passengers to board or alight from a vehicle.

A vehicle track is located on the respective infrastructure link for the mode (railway element of railway network, road element of road network, etc.).

A vehicle stopping place may be served by one or more quays."""@en ;
                      rdfs:label "Vehicle Stopping Place"@en .


###  https://w3id.org/transmodel/facilities#VehicleType
:VehicleType rdf:type owl:Class ;
             rdfs:subClassOf :THINGSTOREVIEW ;
             rdfs:comment "A classification of public transport vehicles according to the vehicle scheduling requirements in mode and capacity"@en ;
             rdfs:label "VehicleType"@en .


###  https://w3id.org/transmodel/facilities#WaitingEquipment
:WaitingEquipment rdf:type owl:Class ;
                  rdfs:subClassOf :SiteEquipment ;
                  rdfs:comment "Specialisation of StopPlaceEquipment for WaitingEquipment (shelter, waiting room, etc.)"@en ;
                  rdfs:label "WaitingEquipment"@en .


###  https://w3id.org/transmodel/facilities#WaitingRoomEquipment
:WaitingRoomEquipment rdf:type owl:Class ;
                      rdfs:subClassOf :WaitingEquipment ,
                                      :WaitingRoomEquipment ;
                      rdfs:comment "A Waiting Room"@en ,
                                   "Specialisation of WaitingEquipment for WaitingRoom, classified by TypeOfWaitingRoom"@en ;
                      rdfs:label "WaitingRoom"@en ,
                                 "WaitingRoomEquipment"@en .


###  https://w3id.org/transmodel/facilities#WheelchairAccessToilet
:WheelchairAccessToilet rdf:type owl:Class ;
                        rdfs:subClassOf :SanitaryEquipment ;
                        rdfs:comment "TODO: Check if this has to be maintained, as it is not present in the Equipment Overview Physical Model of Transmodel (figure 247)"@en .


###  https://w3id.org/transmodel/facilities#WheelchairBabyChange
:WheelchairBabyChange rdf:type owl:Class ;
                      rdfs:subClassOf :SanitaryEquipment ;
                      rdfs:comment "TODO: Check if this has to be maintained, as it is not present in the Equipment Overview Physical Model of Transmodel (figure 247)"@en .


###  https://w3id.org/transmodel/facilities#WheelchairVehicleEquipment
:WheelchairVehicleEquipment rdf:type owl:Class ;
                            rdfs:subClassOf :VehicleEquipment ;
                            rdfs:comment "Specialisation of Vehicle Equipment for wheel chair accessibility on board a Vehicle providing information suchs as the number of wheelchair areas and the access dimmensions"@en ;
                            rdfs:label "WheelchairVehicleEquipment"@en .


###  https://w3id.org/transmodel/journeys#BeaconPoint
<https://w3id.org/transmodel/journeys#BeaconPoint> rdf:type owl:Class ;
                                                   rdfs:subClassOf <https://w3id.org/transmodel/journeys#Point> ;
                                                   rdfs:comment "A Point where a beacon or similar device to support the automatic detection of vehicles passing by is located"@en ;
                                                   rdfs:label "BeaconPoint"@en .


###  https://w3id.org/transmodel/journeys#Point
<https://w3id.org/transmodel/journeys#Point> rdf:type owl:Class ;
                                             rdfs:subClassOf :THINGSTOREVIEW ;
                                             rdfs:label "Point"@en .


###  https://w3id.org/transmodel/journeys#Service
<https://w3id.org/transmodel/journeys#Service> rdf:type owl:Class ;
                                               rdfs:subClassOf :THINGSTOREVIEW ;
                                               rdfs:comment "A ServiceJourney is a Passenger carrying VehicleJourney for one specified DayType. The pattern of working is in principle defined by a ServiceJourneyPattern."@en ,
                                                            "TODO: To remove once that we are sure that we are not breaking anything" ;
                                               rdfs:label "Service"@en .


#################################################################
#    Individuals
#################################################################

###  https://w3id.org/transmodel/facilities#accessible
:accessible rdf:type owl:NamedIndividual .


###  https://w3id.org/transmodel/facilities#audioNavigator
:audioNavigator rdf:type owl:NamedIndividual .


###  https://w3id.org/transmodel/facilities#babychange
:babychange rdf:type owl:NamedIndividual ,
                     :SanitaryEquipment ;
            rdfs:label "babyChange"@en .


###  https://w3id.org/transmodel/facilities#baggageCheckin
:baggageCheckin rdf:type owl:NamedIndividual .


###  https://w3id.org/transmodel/facilities#barrier
:barrier rdf:type owl:NamedIndividual ;
         rdfs:label "barrierEntrance"@en .


###  https://w3id.org/transmodel/facilities#beverageVendingMachine
:beverageVendingMachine rdf:type owl:NamedIndividual .


###  https://w3id.org/transmodel/facilities#bookingHall
:bookingHall rdf:type owl:NamedIndividual ,
                      :PassengerArea ;
             rdfs:label "bookingHall"@en .


###  https://w3id.org/transmodel/facilities#boundedOpenSpace
:boundedOpenSpace rdf:type owl:NamedIndividual ,
                           :PassengerArea .


###  https://w3id.org/transmodel/facilities#buffet
:buffet rdf:type owl:NamedIndividual .


###  https://w3id.org/transmodel/facilities#bunk
:bunk rdf:type owl:NamedIndividual .


###  https://w3id.org/transmodel/facilities#cateringTrolleyService
:cateringTrolleyService rdf:type owl:NamedIndividual .


###  https://w3id.org/transmodel/facilities#compoundTrain
:compoundTrain rdf:type owl:NamedIndividual ,
                        :VehicleType ;
               rdfs:comment "A VehicleType composed of a sequence of more than one vehicles of the type Train"@en ;
               rdfs:label "compoundTrain"@en .


###  https://w3id.org/transmodel/facilities#concourse
:concourse rdf:type owl:NamedIndividual ,
                    :PassengerArea ;
           rdfs:label "concourse"@en .


###  https://w3id.org/transmodel/facilities#confinedSpace
:confinedSpace rdf:type owl:NamedIndividual .


###  https://w3id.org/transmodel/facilities#corridor
:corridor rdf:type owl:NamedIndividual ,
                   :PassengerArea .


###  https://w3id.org/transmodel/facilities#couchette
:couchette rdf:type owl:NamedIndividual .


###  https://w3id.org/transmodel/facilities#crowding
:crowding rdf:type owl:NamedIndividual .


###  https://w3id.org/transmodel/facilities#cycleStorageEquipmentBars
:cycleStorageEquipmentBars rdf:type owl:NamedIndividual .


###  https://w3id.org/transmodel/facilities#cycleStorageEquipmentRacks
:cycleStorageEquipmentRacks rdf:type owl:NamedIndividual .


###  https://w3id.org/transmodel/facilities#cycleStorageEquipmentRailings
:cycleStorageEquipmentRailings rdf:type owl:NamedIndividual .


###  https://w3id.org/transmodel/facilities#directionName
:directionName rdf:type owl:NamedIndividual ,
                        :HeadingSign ;
               rdfs:label "directionName"@en .


###  https://w3id.org/transmodel/facilities#doubleDeck
:doubleDeck rdf:type owl:NamedIndividual ,
                     :VehicleType ;
            rdfs:label "doubleDeck"@en .


###  https://w3id.org/transmodel/facilities#emergencyServiceFirstAid
:emergencyServiceFirstAid rdf:type owl:NamedIndividual .


###  https://w3id.org/transmodel/facilities#emergencyServicePolice
:emergencyServicePolice rdf:type owl:NamedIndividual .


###  https://w3id.org/transmodel/facilities#emergencyServiceSOSPoint
:emergencyServiceSOSPoint rdf:type owl:NamedIndividual .


###  https://w3id.org/transmodel/facilities#emergencyServiceServiceCCTV
:emergencyServiceServiceCCTV rdf:type owl:NamedIndividual .


###  https://w3id.org/transmodel/facilities#entranceEquipmentBarrier
:entranceEquipmentBarrier rdf:type owl:NamedIndividual .


###  https://w3id.org/transmodel/facilities#entranceEquipmentDoor
:entranceEquipmentDoor rdf:type owl:NamedIndividual ;
                       rdfs:label "entranceEquipmentDoor"@en .


###  https://w3id.org/transmodel/facilities#entranceEquipmentRevolvingDoor
:entranceEquipmentRevolvingDoor rdf:type owl:NamedIndividual ;
                                rdfs:label "entranceEquipmentRevolvingDoor"@en .


###  https://w3id.org/transmodel/facilities#equipmentActivated
:equipmentActivated rdf:type owl:NamedIndividual ,
                             :StatusOfEquipment ;
                    rdfs:label "equipmentActivated"@en .


###  https://w3id.org/transmodel/facilities#equipmentAtStopPoint
:equipmentAtStopPoint rdf:type owl:NamedIndividual ;
                      rdfs:label "equipmentAtStopPoint"@en .


###  https://w3id.org/transmodel/facilities#equipmentOnBoard
:equipmentOnBoard rdf:type owl:NamedIndividual .


###  https://w3id.org/transmodel/facilities#equipmentdesactvated
:equipmentdesactvated rdf:type owl:NamedIndividual ,
                               :StatusOfEquipment ;
                      rdfs:label "equipmentDesactivated"@en .


###  https://w3id.org/transmodel/facilities#firstClass
:firstClass rdf:type owl:NamedIndividual .


###  https://w3id.org/transmodel/facilities#foodVendingMachine
:foodVendingMachine rdf:type owl:NamedIndividual .


###  https://w3id.org/transmodel/facilities#full
:full rdf:type owl:NamedIndividual .


###  https://w3id.org/transmodel/facilities#hall
:hall rdf:type owl:NamedIndividual ,
               :PassengerArea .


###  https://w3id.org/transmodel/facilities#handrailOneSide
:handrailOneSide rdf:type owl:NamedIndividual .


###  https://w3id.org/transmodel/facilities#handrailTwoSides
:handrailTwoSides rdf:type owl:NamedIndividual .


###  https://w3id.org/transmodel/facilities#immigrationHall
:immigrationHall rdf:type owl:NamedIndividual ,
                          :PassengerArea ;
                 rdfs:label "immigrationHall"@en .


###  https://w3id.org/transmodel/facilities#incomingCustoms
:incomingCustoms rdf:type owl:NamedIndividual .


###  https://w3id.org/transmodel/facilities#informationDesk
:informationDesk rdf:type owl:NamedIndividual ;
                 rdfs:comment "A public transport information piece of Equipment indoors"@en ;
                 rdfs:label "InformationDesk"@en .


###  https://w3id.org/transmodel/facilities#informationStand
:informationStand rdf:type owl:NamedIndividual ;
                  rdfs:comment "A public transport information piece of Equipment outdoors"@en ;
                  rdfs:label "informationStand"@en .


###  https://w3id.org/transmodel/facilities#lift
:lift rdf:type owl:NamedIndividual .


###  https://w3id.org/transmodel/facilities#lineName
:lineName rdf:type owl:NamedIndividual ,
                   :HeadingSign ;
          rdfs:label "lineName"@en .


###  https://w3id.org/transmodel/facilities#lowFloor
:lowFloor rdf:type owl:NamedIndividual ;
          rdfs:label "lowFloor"@en .


###  https://w3id.org/transmodel/facilities#narrowEntrance
:narrowEntrance rdf:type owl:NamedIndividual ;
                rdfs:label "narrowEntrance"@en .


###  https://w3id.org/transmodel/facilities#noBeveragesAvailable
:noBeveragesAvailable rdf:type owl:NamedIndividual ;
                      rdfs:label ""@en ,
                                 "beverages" .


###  https://w3id.org/transmodel/facilities#noFoodAvailable
:noFoodAvailable rdf:type owl:NamedIndividual ;
                 rdfs:label "food"@en .


###  https://w3id.org/transmodel/facilities#noWaiting
:noWaiting rdf:type owl:NamedIndividual .


###  https://w3id.org/transmodel/facilities#nonAccessible
:nonAccessible rdf:type owl:NamedIndividual .


###  https://w3id.org/transmodel/facilities#outgoingCustoms
:outgoingCustoms rdf:type owl:NamedIndividual .


###  https://w3id.org/transmodel/facilities#placeAccessStairScalator
:placeAccessStairScalator rdf:type owl:NamedIndividual ;
                          rdfs:comment "Specialisation of PlaceAccessStair Equipment dedicated to PlaceAccessStairEscalator"@en ;
                          rdfs:label "placeAccessStairScalator"@en .


###  https://w3id.org/transmodel/facilities#placeAccessStairStair
:placeAccessStairStair rdf:type owl:NamedIndividual ;
                       rdfs:comment "Specialisation of PlaceAccessStair Equipment dedicated to PlaceAccessStairStair"@en ;
                       rdfs:label "placeAccessStairStair"@en .


###  https://w3id.org/transmodel/facilities#placeAccessStairStaircase
:placeAccessStairStaircase rdf:type owl:NamedIndividual ;
                           rdfs:comment "Specialisation of PlaceAccessStair Equipment dedicated to PlaceAccessStairStaircase"@en ;
                           rdfs:label "placeAccessStairStaircase"@en .


###  https://w3id.org/transmodel/facilities#queue
:queue rdf:type owl:NamedIndividual .


###  https://w3id.org/transmodel/facilities#queueManagement
:queueManagement rdf:type owl:NamedIndividual .


###  https://w3id.org/transmodel/facilities#riverFlow
:riverFlow rdf:type owl:NamedIndividual ,
                    :ValidityTrigger ;
           rdfs:label "riverFlow"@en .


###  https://w3id.org/transmodel/facilities#roadClosure
:roadClosure rdf:type owl:NamedIndividual ,
                      :ValidityTrigger ;
             rdfs:label "roadClosure"@en .


###  https://w3id.org/transmodel/facilities#room
:room rdf:type owl:NamedIndividual ,
               :PassengerArea .


###  https://w3id.org/transmodel/facilities#secondClass
:secondClass rdf:type owl:NamedIndividual .


###  https://w3id.org/transmodel/facilities#securityArea
:securityArea rdf:type owl:NamedIndividual ,
                       :PassengerArea ;
              rdfs:label "securityArea"@en .


###  https://w3id.org/transmodel/facilities#shower
:shower rdf:type owl:NamedIndividual ,
                 :SanitaryEquipment .


###  https://w3id.org/transmodel/facilities#snacks
:snacks rdf:type owl:NamedIndividual .


###  https://w3id.org/transmodel/facilities#standardBus
:standardBus rdf:type owl:NamedIndividual ,
                      :VehicleType ;
             rdfs:label "standardBus"@en .


###  https://w3id.org/transmodel/facilities#stepFree
:stepFree rdf:type owl:NamedIndividual ;
          rdfs:label "stepFree"@en .


###  https://w3id.org/transmodel/facilities#taxRefunds
:taxRefunds rdf:type owl:NamedIndividual .


###  https://w3id.org/transmodel/facilities#telematicInformationCenter
:telematicInformationCenter rdf:type owl:NamedIndividual ;
                            rdfs:comment "A public transport information piece of Equipment online"@en ;
                            rdfs:label "telematicInformationService"@en .


###  https://w3id.org/transmodel/facilities#ticketCollection
:ticketCollection rdf:type owl:NamedIndividual .


###  https://w3id.org/transmodel/facilities#ticketPurchase
:ticketPurchase rdf:type owl:NamedIndividual .


###  https://w3id.org/transmodel/facilities#toilet
:toilet rdf:type owl:NamedIndividual ,
                 :SanitaryEquipment .


###  https://w3id.org/transmodel/facilities#visualNavigator
:visualNavigator rdf:type owl:NamedIndividual .


###  https://w3id.org/transmodel/facilities#walkingStick
:walkingStick rdf:type owl:NamedIndividual .


###  https://w3id.org/transmodel/facilities#weatherConditions
:weatherConditions rdf:type owl:NamedIndividual ,
                            :ValidityTrigger ;
                   rdfs:label "weatherConditions"@en .


###  https://w3id.org/transmodel/facilities#wheelchair
:wheelchair rdf:type owl:NamedIndividual .


###  https://w3id.org/transmodel/facilities#wheelchairAccessToilet
:wheelchairAccessToilet rdf:type owl:NamedIndividual ,
                                 :SanitaryEquipment .


###  https://w3id.org/transmodel/facilities#wheelchairBabyChange
:wheelchairBabyChange rdf:type owl:NamedIndividual ,
                               :SanitaryEquipment .


###  https://w3id.org/transmodel/kos/facilities/EquipmentType
<https://w3id.org/transmodel/kos/facilities/EquipmentType> rdf:type owl:NamedIndividual ,
                                                                    <http://www.w3.org/2004/02/skos/core#ConceptScheme> ;
                                                           rdfs:comment "Concept scheme where all the codelists for the types of equipment that are included in the Transmodel ontology are included" .


###  https://w3id.org/transmodel/kos/facilities/FacilityType
<https://w3id.org/transmodel/kos/facilities/FacilityType> rdf:type owl:NamedIndividual ,
                                                                   <http://www.w3.org/2004/02/skos/core#ConceptScheme> ;
                                                          rdfs:comment "Concept scheme where all the codelists for the types of facilities that are included in the Transmodel ontology"@en .


###  https://w3id.org/transmodel/kos/journeys/mobility-limitation
<https://w3id.org/transmodel/kos/journeys/mobility-limitation> rdf:type owl:NamedIndividual ;
                                                               rdfs:comment "List of concepts regarding Mobility Limitation defined in kos/journeys/mobility-limitation"@en .


_:genid115 :mbox "adolfo.anton.bravo@upm.es"@en ;
           :name "Adolfo Anton-Bravo"@en .

#################################################################
#    General axioms
#################################################################

[ rdf:type owl:AllDisjointClasses ;
   owl:members ( :HeadingSign
                 :OtherSign
                 :PlaceSign
               )
 ] .


###  Generated by the OWL API (version 5.1.9) https://github.com/owlcs/owlapi/
